Simplified refinement/soundness proof Termination by counter interpretation (gives reduction order on (ℕ, 0, >)) Ongoing work on reduction closures

Hygge_Theory.thy
@@ -12,92 +12,10 @@ begin
   - Decidability
 *)
 
+fun HeronConf_interpretation :: "(system \<times> instant_index \<times> TESL_formula \<times> TESL_formula) \<Rightarrow> run set" ("\<lbrakk> _ \<rbrakk>\<^sub>H\<^sub>e\<^sub>r\<^sub>o\<^sub>n") where
+  "\<lbrakk> \<Gamma>, n \<turnstile> \<Psi> \<triangleright> \<Phi> \<rbrakk>\<^sub>H\<^sub>e\<^sub>r\<^sub>o\<^sub>n = \<lbrakk>\<lbrakk> \<Gamma> \<rbrakk>\<rbrakk>\<^sub>s\<^sub>y\<^sub>m\<^sub>r\<^sub>u\<^sub>n \<inter> \<lbrakk>\<lbrakk> \<Psi> \<nabla> n \<rbrakk>\<rbrakk>\<^sub>T\<^sub>E\<^sub>S\<^sub>L \<inter> \<lbrakk>\<lbrakk> \<Phi> \<nabla> Suc n \<rbrakk>\<rbrakk>\<^sub>T\<^sub>E\<^sub>S\<^sub>L"
 
 (**) section \<open>Soundness\<close> (**)
-
-(* For each reduction step, the formula [\<psi>] in elimination, produces
-     1. Two primitives         [\<gamma>\<^sub>1] and [\<gamma>\<^sub>2]
-     2. A residual formula     [\<psi>\<^sub>n\<^sub>o\<^sub>w]
-     3. A continuation formula [\<psi>\<^sub>f\<^sub>u\<^sub>t]
-   Their combination is a refinement of the eliminated formula.
-*)
-theorem elimination_soundness:
-  assumes "\<Gamma>, n \<turnstile> \<psi> # \<Psi> \<triangleright> \<Phi>  \<hookrightarrow>  \<gamma>\<^sub>1 # \<gamma>\<^sub>2 # \<Gamma>, n \<turnstile> \<psi>\<^sub>n\<^sub>o\<^sub>w # \<Psi> \<triangleright> \<psi>\<^sub>f\<^sub>u\<^sub>t # \<Phi>"
-  shows "\<lbrakk> \<psi> \<nabla> n \<rbrakk>\<^sub>T\<^sub>E\<^sub>S\<^sub>L \<supseteq> \<lbrakk> \<gamma>\<^sub>1 \<rbrakk>\<^sub>s\<^sub>y\<^sub>m\<^sub>r\<^sub>u\<^sub>n \<inter> \<lbrakk> \<gamma>\<^sub>2 \<rbrakk>\<^sub>s\<^sub>y\<^sub>m\<^sub>r\<^sub>u\<^sub>n \<inter> \<lbrakk> \<psi>\<^sub>n\<^sub>o\<^sub>w \<nabla> n \<rbrakk>\<^sub>T\<^sub>E\<^sub>S\<^sub>L \<inter> \<lbrakk> \<psi>\<^sub>f\<^sub>u\<^sub>t \<nabla> Suc n \<rbrakk>\<^sub>T\<^sub>E\<^sub>S\<^sub>L"
-  proof (insert assms, erule operational_semantics_step.cases)
-    show "\<And>\<Gamma>' na \<Phi>'.
-       (\<Gamma>, n \<turnstile> \<psi> # \<Psi> \<triangleright> \<Phi>) = (\<Gamma>', na \<turnstile> [] \<triangleright> \<Phi>') \<Longrightarrow>
-       (\<gamma>\<^sub>1 # \<gamma>\<^sub>2 # \<Gamma>, n \<turnstile> \<psi>\<^sub>n\<^sub>o\<^sub>w # \<Psi> \<triangleright> \<psi>\<^sub>f\<^sub>u\<^sub>t # \<Phi>) = (\<Gamma>', Suc na \<turnstile> \<Phi>' \<triangleright> []) \<Longrightarrow>
-       consistent_run \<Gamma>' \<Longrightarrow>
-       \<lbrakk> \<gamma>\<^sub>1 \<rbrakk>\<^sub>s\<^sub>y\<^sub>m\<^sub>r\<^sub>u\<^sub>n \<inter> \<lbrakk> \<gamma>\<^sub>2 \<rbrakk>\<^sub>s\<^sub>y\<^sub>m\<^sub>r\<^sub>u\<^sub>n \<inter> \<lbrakk> \<psi>\<^sub>n\<^sub>o\<^sub>w \<nabla> n \<rbrakk>\<^sub>T\<^sub>E\<^sub>S\<^sub>L \<inter> \<lbrakk> \<psi>\<^sub>f\<^sub>u\<^sub>t \<nabla> Suc n \<rbrakk>\<^sub>T\<^sub>E\<^sub>S\<^sub>L \<subseteq> \<lbrakk> \<psi> \<nabla> n \<rbrakk>\<^sub>T\<^sub>E\<^sub>S\<^sub>L"
-      by simp
-    show "\<And>\<Gamma>' na K \<tau> \<Psi>' \<Phi>'.
-       (\<Gamma>, n \<turnstile> \<psi> # \<Psi> \<triangleright> \<Phi>) = (\<Gamma>', na \<turnstile> (K sporadic \<tau>) # \<Psi>' \<triangleright> \<Phi>') \<Longrightarrow>
-       (\<gamma>\<^sub>1 # \<gamma>\<^sub>2 # \<Gamma>, n \<turnstile> \<psi>\<^sub>n\<^sub>o\<^sub>w # \<Psi> \<triangleright> \<psi>\<^sub>f\<^sub>u\<^sub>t # \<Phi>) = (\<top>\<^sub>s\<^sub>y\<^sub>m\<^sub>r\<^sub>u\<^sub>n # \<top>\<^sub>s\<^sub>y\<^sub>m\<^sub>r\<^sub>u\<^sub>n # \<Gamma>', na \<turnstile> \<top>\<^sub>T\<^sub>E\<^sub>S\<^sub>L # \<Psi>' \<triangleright> (K sporadic \<tau>) # \<Phi>') \<Longrightarrow>
-       consistent_run \<Gamma>' \<Longrightarrow>
-       \<lbrakk> \<gamma>\<^sub>1 \<rbrakk>\<^sub>s\<^sub>y\<^sub>m\<^sub>r\<^sub>u\<^sub>n \<inter> \<lbrakk> \<gamma>\<^sub>2 \<rbrakk>\<^sub>s\<^sub>y\<^sub>m\<^sub>r\<^sub>u\<^sub>n \<inter> \<lbrakk> \<psi>\<^sub>n\<^sub>o\<^sub>w \<nabla> n \<rbrakk>\<^sub>T\<^sub>E\<^sub>S\<^sub>L \<inter> \<lbrakk> \<psi>\<^sub>f\<^sub>u\<^sub>t \<nabla> Suc n \<rbrakk>\<^sub>T\<^sub>E\<^sub>S\<^sub>L \<subseteq> \<lbrakk> \<psi> \<nabla> n \<rbrakk>\<^sub>T\<^sub>E\<^sub>S\<^sub>L"
-      using TESL_interp_at_index_sporadic_cases by blast
-    show "\<And>K na \<tau> \<Gamma>' \<Psi>' \<Phi>'.
-       (\<Gamma>, n \<turnstile> \<psi> # \<Psi> \<triangleright> \<Phi>) = (\<Gamma>', na \<turnstile> (K sporadic \<tau>) # \<Psi>' \<triangleright> \<Phi>') \<Longrightarrow>
-       (\<gamma>\<^sub>1 # \<gamma>\<^sub>2 # \<Gamma>, n \<turnstile> \<psi>\<^sub>n\<^sub>o\<^sub>w # \<Psi> \<triangleright> \<psi>\<^sub>f\<^sub>u\<^sub>t # \<Phi>) = (K \<Up> na # K \<Down> na @ \<lfloor> \<tau> \<rfloor> # \<Gamma>', na \<turnstile> \<top>\<^sub>T\<^sub>E\<^sub>S\<^sub>L # \<Psi>' \<triangleright> \<top>\<^sub>T\<^sub>E\<^sub>S\<^sub>L # \<Phi>') \<Longrightarrow>
-       consistent_run (K \<Up> na # K \<Down> na @ \<lfloor> \<tau> \<rfloor> # \<Gamma>') \<Longrightarrow>
-       \<lbrakk> \<gamma>\<^sub>1 \<rbrakk>\<^sub>s\<^sub>y\<^sub>m\<^sub>r\<^sub>u\<^sub>n \<inter> \<lbrakk> \<gamma>\<^sub>2 \<rbrakk>\<^sub>s\<^sub>y\<^sub>m\<^sub>r\<^sub>u\<^sub>n \<inter> \<lbrakk> \<psi>\<^sub>n\<^sub>o\<^sub>w \<nabla> n \<rbrakk>\<^sub>T\<^sub>E\<^sub>S\<^sub>L \<inter> \<lbrakk> \<psi>\<^sub>f\<^sub>u\<^sub>t \<nabla> Suc n \<rbrakk>\<^sub>T\<^sub>E\<^sub>S\<^sub>L \<subseteq> \<lbrakk> \<psi> \<nabla> n \<rbrakk>\<^sub>T\<^sub>E\<^sub>S\<^sub>L"
-      using TESL_interp_at_index_sporadic_cases by blast
-    show "\<And>\<Gamma>' na K\<^sub>1 \<tau> K\<^sub>2 \<Psi>' \<Phi>'.
-       (\<Gamma>, n \<turnstile> \<psi> # \<Psi> \<triangleright> \<Phi>) = (\<Gamma>', na \<turnstile> (K\<^sub>1 sporadic \<tau> on K\<^sub>2) # \<Psi>' \<triangleright> \<Phi>') \<Longrightarrow>
-       (\<gamma>\<^sub>1 # \<gamma>\<^sub>2 # \<Gamma>, n \<turnstile> \<psi>\<^sub>n\<^sub>o\<^sub>w # \<Psi> \<triangleright> \<psi>\<^sub>f\<^sub>u\<^sub>t # \<Phi>) = (\<top>\<^sub>s\<^sub>y\<^sub>m\<^sub>r\<^sub>u\<^sub>n # \<top>\<^sub>s\<^sub>y\<^sub>m\<^sub>r\<^sub>u\<^sub>n # \<Gamma>', na \<turnstile> \<top>\<^sub>T\<^sub>E\<^sub>S\<^sub>L # \<Psi>' \<triangleright> (K\<^sub>1 sporadic \<tau> on K\<^sub>2) # \<Phi>') \<Longrightarrow>
-       consistent_run \<Gamma>' \<Longrightarrow>
-       \<lbrakk> \<gamma>\<^sub>1 \<rbrakk>\<^sub>s\<^sub>y\<^sub>m\<^sub>r\<^sub>u\<^sub>n \<inter> \<lbrakk> \<gamma>\<^sub>2 \<rbrakk>\<^sub>s\<^sub>y\<^sub>m\<^sub>r\<^sub>u\<^sub>n \<inter> \<lbrakk> \<psi>\<^sub>n\<^sub>o\<^sub>w \<nabla> n \<rbrakk>\<^sub>T\<^sub>E\<^sub>S\<^sub>L \<inter> \<lbrakk> \<psi>\<^sub>f\<^sub>u\<^sub>t \<nabla> Suc n \<rbrakk>\<^sub>T\<^sub>E\<^sub>S\<^sub>L \<subseteq> \<lbrakk> \<psi> \<nabla> n \<rbrakk>\<^sub>T\<^sub>E\<^sub>S\<^sub>L"
-      using TESL_interp_at_index_sporadicon_cases by blast
-    show "\<And>K\<^sub>1 na K\<^sub>2 \<tau> \<Gamma>' \<Psi>' \<Phi>'.
-       (\<Gamma>, n \<turnstile> \<psi> # \<Psi> \<triangleright> \<Phi>) = (\<Gamma>', na \<turnstile> (K\<^sub>1 sporadic \<tau> on K\<^sub>2) # \<Psi>' \<triangleright> \<Phi>') \<Longrightarrow>
-       (\<gamma>\<^sub>1 # \<gamma>\<^sub>2 # \<Gamma>, n \<turnstile> \<psi>\<^sub>n\<^sub>o\<^sub>w # \<Psi> \<triangleright> \<psi>\<^sub>f\<^sub>u\<^sub>t # \<Phi>) =
-       (K\<^sub>1 \<Up> na # K\<^sub>2 \<Down> na @ \<tau> # \<Gamma>', na \<turnstile> \<top>\<^sub>T\<^sub>E\<^sub>S\<^sub>L # \<Psi>' \<triangleright> \<top>\<^sub>T\<^sub>E\<^sub>S\<^sub>L # \<Phi>') \<Longrightarrow>
-       consistent_run (K\<^sub>1 \<Up> na # K\<^sub>2 \<Down> na @ \<tau> # \<Gamma>') \<Longrightarrow>
-       \<lbrakk> \<gamma>\<^sub>1 \<rbrakk>\<^sub>s\<^sub>y\<^sub>m\<^sub>r\<^sub>u\<^sub>n \<inter> \<lbrakk> \<gamma>\<^sub>2 \<rbrakk>\<^sub>s\<^sub>y\<^sub>m\<^sub>r\<^sub>u\<^sub>n \<inter> \<lbrakk> \<psi>\<^sub>n\<^sub>o\<^sub>w \<nabla> n \<rbrakk>\<^sub>T\<^sub>E\<^sub>S\<^sub>L \<inter> \<lbrakk> \<psi>\<^sub>f\<^sub>u\<^sub>t \<nabla> Suc n \<rbrakk>\<^sub>T\<^sub>E\<^sub>S\<^sub>L \<subseteq> \<lbrakk> \<psi> \<nabla> n \<rbrakk>\<^sub>T\<^sub>E\<^sub>S\<^sub>L"
-      using TESL_interp_at_index_sporadicon_cases by blast
-    show "\<And>K\<^sub>1 na \<alpha> K\<^sub>2 \<beta> \<Gamma>' \<Psi>' \<Phi>'.
-       (\<Gamma>, n \<turnstile> \<psi> # \<Psi> \<triangleright> \<Phi>) = (\<Gamma>', na \<turnstile> (tag-relation K\<^sub>1 = \<alpha> * K\<^sub>2 + \<beta>) # \<Psi>' \<triangleright> \<Phi>') \<Longrightarrow>
-       (\<gamma>\<^sub>1 # \<gamma>\<^sub>2 # \<Gamma>, n \<turnstile> \<psi>\<^sub>n\<^sub>o\<^sub>w # \<Psi> \<triangleright> \<psi>\<^sub>f\<^sub>u\<^sub>t # \<Phi>) =
-       (\<top>\<^sub>s\<^sub>y\<^sub>m\<^sub>r\<^sub>u\<^sub>n #
-        \<tau>\<^sub>v\<^sub>a\<^sub>r (K\<^sub>1, na) \<doteq> \<alpha> * \<tau>\<^sub>v\<^sub>a\<^sub>r (K\<^sub>2, na) + \<beta> #
-        \<Gamma>', na \<turnstile> \<top>\<^sub>T\<^sub>E\<^sub>S\<^sub>L # \<Psi>' \<triangleright> (tag-relation K\<^sub>1 = \<alpha> * K\<^sub>2 + \<beta>) # \<Phi>') \<Longrightarrow>
-       consistent_run (\<tau>\<^sub>v\<^sub>a\<^sub>r (K\<^sub>1, na) \<doteq> \<alpha> * \<tau>\<^sub>v\<^sub>a\<^sub>r (K\<^sub>2, na) + \<beta> # \<Gamma>') \<Longrightarrow>
-       \<lbrakk> \<gamma>\<^sub>1 \<rbrakk>\<^sub>s\<^sub>y\<^sub>m\<^sub>r\<^sub>u\<^sub>n \<inter> \<lbrakk> \<gamma>\<^sub>2 \<rbrakk>\<^sub>s\<^sub>y\<^sub>m\<^sub>r\<^sub>u\<^sub>n \<inter> \<lbrakk> \<psi>\<^sub>n\<^sub>o\<^sub>w \<nabla> n \<rbrakk>\<^sub>T\<^sub>E\<^sub>S\<^sub>L \<inter> \<lbrakk> \<psi>\<^sub>f\<^sub>u\<^sub>t \<nabla> Suc n \<rbrakk>\<^sub>T\<^sub>E\<^sub>S\<^sub>L \<subseteq> \<lbrakk> \<psi> \<nabla> n \<rbrakk>\<^sub>T\<^sub>E\<^sub>S\<^sub>L"
-      using TESL_interp_at_index_tagrel_cases by blast
-    show "\<And>K\<^sub>1 na \<Gamma>' K\<^sub>2 \<Psi>' \<Phi>'.
-       (\<Gamma>, n \<turnstile> \<psi> # \<Psi> \<triangleright> \<Phi>) = (\<Gamma>', na \<turnstile> (K\<^sub>1 implies K\<^sub>2) # \<Psi>' \<triangleright> \<Phi>') \<Longrightarrow>
-       (\<gamma>\<^sub>1 # \<gamma>\<^sub>2 # \<Gamma>, n \<turnstile> \<psi>\<^sub>n\<^sub>o\<^sub>w # \<Psi> \<triangleright> \<psi>\<^sub>f\<^sub>u\<^sub>t # \<Phi>) =
-       (\<top>\<^sub>s\<^sub>y\<^sub>m\<^sub>r\<^sub>u\<^sub>n # K\<^sub>1 \<not>\<Up> na # \<Gamma>', na \<turnstile> \<top>\<^sub>T\<^sub>E\<^sub>S\<^sub>L # \<Psi>' \<triangleright> (K\<^sub>1 implies K\<^sub>2) # \<Phi>') \<Longrightarrow>
-       consistent_run (K\<^sub>1 \<not>\<Up> na # \<Gamma>') \<Longrightarrow>
-       \<lbrakk> \<gamma>\<^sub>1 \<rbrakk>\<^sub>s\<^sub>y\<^sub>m\<^sub>r\<^sub>u\<^sub>n \<inter> \<lbrakk> \<gamma>\<^sub>2 \<rbrakk>\<^sub>s\<^sub>y\<^sub>m\<^sub>r\<^sub>u\<^sub>n \<inter> \<lbrakk> \<psi>\<^sub>n\<^sub>o\<^sub>w \<nabla> n \<rbrakk>\<^sub>T\<^sub>E\<^sub>S\<^sub>L \<inter> \<lbrakk> \<psi>\<^sub>f\<^sub>u\<^sub>t \<nabla> Suc n \<rbrakk>\<^sub>T\<^sub>E\<^sub>S\<^sub>L \<subseteq> \<lbrakk> \<psi> \<nabla> n \<rbrakk>\<^sub>T\<^sub>E\<^sub>S\<^sub>L"
-      using TESL_interp_at_index_implies_cases by blast
-    show "\<And>K\<^sub>1 na K\<^sub>2 \<Gamma>' \<Psi>' \<Phi>'.
-       (\<Gamma>, n \<turnstile> \<psi> # \<Psi> \<triangleright> \<Phi>) = (\<Gamma>', na \<turnstile> (K\<^sub>1 implies K\<^sub>2) # \<Psi>' \<triangleright> \<Phi>') \<Longrightarrow>
-       (\<gamma>\<^sub>1 # \<gamma>\<^sub>2 # \<Gamma>, n \<turnstile> \<psi>\<^sub>n\<^sub>o\<^sub>w # \<Psi> \<triangleright> \<psi>\<^sub>f\<^sub>u\<^sub>t # \<Phi>) = (K\<^sub>1 \<Up> na # K\<^sub>2 \<Up> na # \<Gamma>', na \<turnstile> \<top>\<^sub>T\<^sub>E\<^sub>S\<^sub>L # \<Psi>' \<triangleright> (K\<^sub>1 implies K\<^sub>2) # \<Phi>') \<Longrightarrow>
-       consistent_run (K\<^sub>1 \<Up> na # K\<^sub>2 \<Up> na # \<Gamma>') \<Longrightarrow>
-       \<lbrakk> \<gamma>\<^sub>1 \<rbrakk>\<^sub>s\<^sub>y\<^sub>m\<^sub>r\<^sub>u\<^sub>n \<inter> \<lbrakk> \<gamma>\<^sub>2 \<rbrakk>\<^sub>s\<^sub>y\<^sub>m\<^sub>r\<^sub>u\<^sub>n \<inter> \<lbrakk> \<psi>\<^sub>n\<^sub>o\<^sub>w \<nabla> n \<rbrakk>\<^sub>T\<^sub>E\<^sub>S\<^sub>L \<inter> \<lbrakk> \<psi>\<^sub>f\<^sub>u\<^sub>t \<nabla> Suc n \<rbrakk>\<^sub>T\<^sub>E\<^sub>S\<^sub>L \<subseteq> \<lbrakk> \<psi> \<nabla> n \<rbrakk>\<^sub>T\<^sub>E\<^sub>S\<^sub>L"
-      using TESL_interp_at_index_implies_cases by blast
-    show "\<And>K\<^sub>1 na \<Gamma>' \<delta>\<tau> K\<^sub>2 K\<^sub>3 \<Psi>' \<Phi>'.
-       (\<Gamma>, n \<turnstile> \<psi> # \<Psi> \<triangleright> \<Phi>) = (\<Gamma>', na \<turnstile> (K\<^sub>1 time-delayed by \<delta>\<tau> on K\<^sub>2 implies K\<^sub>3) # \<Psi>' \<triangleright> \<Phi>') \<Longrightarrow>
-       (\<gamma>\<^sub>1 # \<gamma>\<^sub>2 # \<Gamma>, n \<turnstile> \<psi>\<^sub>n\<^sub>o\<^sub>w # \<Psi> \<triangleright> \<psi>\<^sub>f\<^sub>u\<^sub>t # \<Phi>) = (\<top>\<^sub>s\<^sub>y\<^sub>m\<^sub>r\<^sub>u\<^sub>n # K\<^sub>1 \<not>\<Up> na # \<Gamma>', na \<turnstile> \<top>\<^sub>T\<^sub>E\<^sub>S\<^sub>L # \<Psi>' \<triangleright> (K\<^sub>1 time-delayed by \<delta>\<tau> on K\<^sub>2 implies K\<^sub>3) # \<Phi>') \<Longrightarrow>
-       consistent_run (K\<^sub>1 \<not>\<Up> na # \<Gamma>') \<Longrightarrow>
-       \<lbrakk> \<gamma>\<^sub>1 \<rbrakk>\<^sub>s\<^sub>y\<^sub>m\<^sub>r\<^sub>u\<^sub>n \<inter> \<lbrakk> \<gamma>\<^sub>2 \<rbrakk>\<^sub>s\<^sub>y\<^sub>m\<^sub>r\<^sub>u\<^sub>n \<inter> \<lbrakk> \<psi>\<^sub>n\<^sub>o\<^sub>w \<nabla> n \<rbrakk>\<^sub>T\<^sub>E\<^sub>S\<^sub>L \<inter> \<lbrakk> \<psi>\<^sub>f\<^sub>u\<^sub>t \<nabla> Suc n \<rbrakk>\<^sub>T\<^sub>E\<^sub>S\<^sub>L \<subseteq> \<lbrakk> \<psi> \<nabla> n \<rbrakk>\<^sub>T\<^sub>E\<^sub>S\<^sub>L"
-      using TESL_interp_at_index_timedelayed_cases by blast
-    show "\<And>K\<^sub>1 na \<Gamma>' \<delta>\<tau> K\<^sub>2 K\<^sub>3 \<Psi>' \<Phi>'.
-       (\<Gamma>, n \<turnstile> \<psi> # \<Psi> \<triangleright> \<Phi>) = (\<Gamma>', na \<turnstile> (K\<^sub>1 time-delayed by \<delta>\<tau> on K\<^sub>2 implies K\<^sub>3) # \<Psi>' \<triangleright> \<Phi>') \<Longrightarrow>
-       (\<gamma>\<^sub>1 # \<gamma>\<^sub>2 # \<Gamma>, n \<turnstile> \<psi>\<^sub>n\<^sub>o\<^sub>w # \<Psi> \<triangleright> \<psi>\<^sub>f\<^sub>u\<^sub>t # \<Phi>)
-         = (\<top>\<^sub>s\<^sub>y\<^sub>m\<^sub>r\<^sub>u\<^sub>n # K\<^sub>1 \<Up> na # \<Gamma>', na \<turnstile> (K\<^sub>3 sporadic \<lfloor> \<tau>\<^sub>v\<^sub>a\<^sub>r (K\<^sub>2, na) \<oplus> \<delta>\<tau> \<rfloor> on K\<^sub>2) # \<Psi>' \<triangleright> (K\<^sub>1 time-delayed by \<delta>\<tau> on K\<^sub>2 implies K\<^sub>3) # \<Phi>') \<Longrightarrow>
-       consistent_run (K\<^sub>1 \<Up> na # \<Gamma>') \<Longrightarrow>
-       \<lbrakk> \<gamma>\<^sub>1 \<rbrakk>\<^sub>s\<^sub>y\<^sub>m\<^sub>r\<^sub>u\<^sub>n \<inter> \<lbrakk> \<gamma>\<^sub>2 \<rbrakk>\<^sub>s\<^sub>y\<^sub>m\<^sub>r\<^sub>u\<^sub>n \<inter> \<lbrakk> \<psi>\<^sub>n\<^sub>o\<^sub>w \<nabla> n \<rbrakk>\<^sub>T\<^sub>E\<^sub>S\<^sub>L \<inter> \<lbrakk> \<psi>\<^sub>f\<^sub>u\<^sub>t \<nabla> Suc n \<rbrakk>\<^sub>T\<^sub>E\<^sub>S\<^sub>L \<subseteq> \<lbrakk> \<psi> \<nabla> n \<rbrakk>\<^sub>T\<^sub>E\<^sub>S\<^sub>L"
-      using TESL_interp_at_index_timedelayed_cases by blast
-  qed
-
-lemma elimination_refinement:
-  assumes "\<Gamma>, n \<turnstile> \<psi> # \<Psi> \<triangleright> \<Phi>  \<hookrightarrow>  \<gamma>\<^sub>1 # \<gamma>\<^sub>2 # \<Gamma>, n \<turnstile> \<psi>\<^sub>n\<^sub>o\<^sub>w # \<Psi> \<triangleright> \<psi>\<^sub>f\<^sub>u\<^sub>t # \<Phi>"
-  shows "\<lbrakk>\<lbrakk> \<Gamma> \<rbrakk>\<rbrakk>\<^sub>s\<^sub>y\<^sub>m\<^sub>r\<^sub>u\<^sub>n \<inter> \<lbrakk> \<psi> \<nabla> n \<rbrakk>\<^sub>T\<^sub>E\<^sub>S\<^sub>L \<inter> \<lbrakk>\<lbrakk> \<Psi> \<nabla> n \<rbrakk>\<rbrakk>\<^sub>T\<^sub>E\<^sub>S\<^sub>L \<inter> \<lbrakk>\<lbrakk> \<Phi> \<nabla> Suc n \<rbrakk>\<rbrakk>\<^sub>T\<^sub>E\<^sub>S\<^sub>L
-          \<supseteq> \<lbrakk> \<gamma>\<^sub>1 \<rbrakk>\<^sub>s\<^sub>y\<^sub>m\<^sub>r\<^sub>u\<^sub>n \<inter> \<lbrakk> \<gamma>\<^sub>2 \<rbrakk>\<^sub>s\<^sub>y\<^sub>m\<^sub>r\<^sub>u\<^sub>n \<inter> \<lbrakk>\<lbrakk> \<Gamma> \<rbrakk>\<rbrakk>\<^sub>s\<^sub>y\<^sub>m\<^sub>r\<^sub>u\<^sub>n \<inter> \<lbrakk> \<psi>\<^sub>n\<^sub>o\<^sub>w \<nabla> n \<rbrakk>\<^sub>T\<^sub>E\<^sub>S\<^sub>L \<inter> \<lbrakk>\<lbrakk> \<Psi> \<nabla> n \<rbrakk>\<rbrakk>\<^sub>T\<^sub>E\<^sub>S\<^sub>L \<inter> \<lbrakk> \<psi>\<^sub>f\<^sub>u\<^sub>t \<nabla> Suc n \<rbrakk>\<^sub>T\<^sub>E\<^sub>S\<^sub>L \<inter> \<lbrakk>\<lbrakk> \<Phi> \<nabla> Suc n \<rbrakk>\<rbrakk>\<^sub>T\<^sub>E\<^sub>S\<^sub>L"
-  using assms elimination_soundness by blast
 
 theorem reduction_refinement:
   assumes "\<Gamma>\<^sub>1, n\<^sub>1 \<turnstile> \<Psi>\<^sub>1 \<triangleright> \<Phi>\<^sub>1  \<hookrightarrow>  \<Gamma>\<^sub>2, n\<^sub>2 \<turnstile> \<Psi>\<^sub>2 \<triangleright> \<Phi>\<^sub>2"
@@ -111,65 +29,217 @@ theorem reduction_refinement:
     by auto
   show "\<And>\<Gamma> n K \<tau> \<Psi> \<Phi>.
        (\<Gamma>\<^sub>1, n\<^sub>1 \<turnstile> \<Psi>\<^sub>1 \<triangleright> \<Phi>\<^sub>1) = (\<Gamma>, n \<turnstile> (K sporadic \<tau>) # \<Psi> \<triangleright> \<Phi>) \<Longrightarrow>
-       (\<Gamma>\<^sub>2, n\<^sub>2 \<turnstile> \<Psi>\<^sub>2 \<triangleright> \<Phi>\<^sub>2) = (\<top>\<^sub>s\<^sub>y\<^sub>m\<^sub>r\<^sub>u\<^sub>n # \<top>\<^sub>s\<^sub>y\<^sub>m\<^sub>r\<^sub>u\<^sub>n # \<Gamma>, n \<turnstile> \<top>\<^sub>T\<^sub>E\<^sub>S\<^sub>L # \<Psi> \<triangleright> (K sporadic \<tau>) # \<Phi>) \<Longrightarrow>
+       (\<Gamma>\<^sub>2, n\<^sub>2 \<turnstile> \<Psi>\<^sub>2 \<triangleright> \<Phi>\<^sub>2) = (\<Gamma>, n \<turnstile> \<Psi> \<triangleright> (K sporadic \<tau>) # \<Phi>) \<Longrightarrow>
        consistent_run \<Gamma> \<Longrightarrow>
        \<lbrakk>\<lbrakk> \<Gamma>\<^sub>2 \<rbrakk>\<rbrakk>\<^sub>s\<^sub>y\<^sub>m\<^sub>r\<^sub>u\<^sub>n \<inter> \<lbrakk>\<lbrakk> \<Psi>\<^sub>2 \<nabla> n\<^sub>2 \<rbrakk>\<rbrakk>\<^sub>T\<^sub>E\<^sub>S\<^sub>L \<inter> \<lbrakk>\<lbrakk> \<Phi>\<^sub>2 \<nabla> Suc n\<^sub>2 \<rbrakk>\<rbrakk>\<^sub>T\<^sub>E\<^sub>S\<^sub>L \<subseteq> \<lbrakk>\<lbrakk> \<Gamma>\<^sub>1 \<rbrakk>\<rbrakk>\<^sub>s\<^sub>y\<^sub>m\<^sub>r\<^sub>u\<^sub>n \<inter> \<lbrakk>\<lbrakk> \<Psi>\<^sub>1 \<nabla> n\<^sub>1 \<rbrakk>\<rbrakk>\<^sub>T\<^sub>E\<^sub>S\<^sub>L \<inter> \<lbrakk>\<lbrakk> \<Phi>\<^sub>1 \<nabla> Suc n\<^sub>1 \<rbrakk>\<rbrakk>\<^sub>T\<^sub>E\<^sub>S\<^sub>L"
-    using elimination_refinement
-    by (metis (no_types, lifting) Pair_inject TESL_interpretation_at_index_cons_morph assms inf_sup_aci(2) symbolic_run_interpretation.simps(2))
+    using TESL_interp_at_index_sporadic_cases
+    by (smt Int_subset_iff Pair_inject TESL_interpretation_at_index_cons_morph inf.cobounded1 inf.cobounded2 subset_trans sup.cobounded2)
   show "\<And>K n \<tau> \<Gamma> \<Psi> \<Phi>.
        (\<Gamma>\<^sub>1, n\<^sub>1 \<turnstile> \<Psi>\<^sub>1 \<triangleright> \<Phi>\<^sub>1) = (\<Gamma>, n \<turnstile> (K sporadic \<tau>) # \<Psi> \<triangleright> \<Phi>) \<Longrightarrow>
-       (\<Gamma>\<^sub>2, n\<^sub>2 \<turnstile> \<Psi>\<^sub>2 \<triangleright> \<Phi>\<^sub>2) = (K \<Up> n # K \<Down> n @ \<lfloor> \<tau> \<rfloor> # \<Gamma>, n \<turnstile> \<top>\<^sub>T\<^sub>E\<^sub>S\<^sub>L # \<Psi> \<triangleright> \<top>\<^sub>T\<^sub>E\<^sub>S\<^sub>L # \<Phi>) \<Longrightarrow>
+       (\<Gamma>\<^sub>2, n\<^sub>2 \<turnstile> \<Psi>\<^sub>2 \<triangleright> \<Phi>\<^sub>2) = (K \<Up> n # K \<Down> n @ \<lfloor> \<tau> \<rfloor> # \<Gamma>, n \<turnstile> \<Psi> \<triangleright> \<Phi>) \<Longrightarrow>
        consistent_run (K \<Up> n # K \<Down> n @ \<lfloor> \<tau> \<rfloor> # \<Gamma>) \<Longrightarrow>
        \<lbrakk>\<lbrakk> \<Gamma>\<^sub>2 \<rbrakk>\<rbrakk>\<^sub>s\<^sub>y\<^sub>m\<^sub>r\<^sub>u\<^sub>n \<inter> \<lbrakk>\<lbrakk> \<Psi>\<^sub>2 \<nabla> n\<^sub>2 \<rbrakk>\<rbrakk>\<^sub>T\<^sub>E\<^sub>S\<^sub>L \<inter> \<lbrakk>\<lbrakk> \<Phi>\<^sub>2 \<nabla> Suc n\<^sub>2 \<rbrakk>\<rbrakk>\<^sub>T\<^sub>E\<^sub>S\<^sub>L \<subseteq> \<lbrakk>\<lbrakk> \<Gamma>\<^sub>1 \<rbrakk>\<rbrakk>\<^sub>s\<^sub>y\<^sub>m\<^sub>r\<^sub>u\<^sub>n \<inter> \<lbrakk>\<lbrakk> \<Psi>\<^sub>1 \<nabla> n\<^sub>1 \<rbrakk>\<rbrakk>\<^sub>T\<^sub>E\<^sub>S\<^sub>L \<inter> \<lbrakk>\<lbrakk> \<Phi>\<^sub>1 \<nabla> Suc n\<^sub>1 \<rbrakk>\<rbrakk>\<^sub>T\<^sub>E\<^sub>S\<^sub>L"
-    using elimination_refinement by auto
+    using TESL_interp_at_index_sporadic_cases
+  proof -
+    fix K :: clock and n :: nat and \<tau> :: tag_const and \<Gamma> :: "constr list" and \<Psi> :: "TESL_atomic list" and \<Phi> :: "TESL_atomic list"
+    assume a1: "(\<Gamma>\<^sub>2, n\<^sub>2 \<turnstile> \<Psi>\<^sub>2 \<triangleright> \<Phi>\<^sub>2) = (K \<Up> n # K \<Down> n @ \<lfloor> \<tau> \<rfloor> # \<Gamma>, n \<turnstile> \<Psi> \<triangleright> \<Phi>)"
+    assume a2: "(\<Gamma>\<^sub>1, n\<^sub>1 \<turnstile> \<Psi>\<^sub>1 \<triangleright> \<Phi>\<^sub>1) = (\<Gamma>, n \<turnstile> (K sporadic \<tau>) # \<Psi> \<triangleright> \<Phi>)"
+    have f3: "\<lbrakk> K \<Up> n \<rbrakk>\<^sub>s\<^sub>y\<^sub>m\<^sub>r\<^sub>u\<^sub>n \<inter> (\<lbrakk> K \<Down> n @ \<lfloor> \<tau> \<rfloor> \<rbrakk>\<^sub>s\<^sub>y\<^sub>m\<^sub>r\<^sub>u\<^sub>n \<inter> \<lbrakk>\<lbrakk> \<Gamma> \<rbrakk>\<rbrakk>\<^sub>s\<^sub>y\<^sub>m\<^sub>r\<^sub>u\<^sub>n) = \<lbrakk>\<lbrakk> \<Gamma>\<^sub>2 \<rbrakk>\<rbrakk>\<^sub>s\<^sub>y\<^sub>m\<^sub>r\<^sub>u\<^sub>n"
+      using a1 by force
+    have "(\<lbrakk> K \<Up> n \<rbrakk>\<^sub>s\<^sub>y\<^sub>m\<^sub>r\<^sub>u\<^sub>n \<inter> \<lbrakk> K \<Down> n @ \<lfloor> \<tau> \<rfloor> \<rbrakk>\<^sub>s\<^sub>y\<^sub>m\<^sub>r\<^sub>u\<^sub>n \<union> \<lbrakk> K sporadic \<tau> \<nabla> Suc n \<rbrakk>\<^sub>T\<^sub>E\<^sub>S\<^sub>L) \<inter> \<lbrakk>\<lbrakk> \<Psi>\<^sub>2 \<nabla> n\<^sub>2 \<rbrakk>\<rbrakk>\<^sub>T\<^sub>E\<^sub>S\<^sub>L = \<lbrakk>\<lbrakk> \<Psi>\<^sub>1 \<nabla> n\<^sub>1 \<rbrakk>\<rbrakk>\<^sub>T\<^sub>E\<^sub>S\<^sub>L"
+      using a2 a1 by (metis (no_types) Pair_inject TESL_interp_at_index_sporadic_cases TESL_interpretation_at_index_cons_morph)
+    then show "\<lbrakk>\<lbrakk> \<Gamma>\<^sub>2 \<rbrakk>\<rbrakk>\<^sub>s\<^sub>y\<^sub>m\<^sub>r\<^sub>u\<^sub>n \<inter> \<lbrakk>\<lbrakk> \<Psi>\<^sub>2 \<nabla> n\<^sub>2 \<rbrakk>\<rbrakk>\<^sub>T\<^sub>E\<^sub>S\<^sub>L \<inter> \<lbrakk>\<lbrakk> \<Phi>\<^sub>2 \<nabla> Suc n\<^sub>2 \<rbrakk>\<rbrakk>\<^sub>T\<^sub>E\<^sub>S\<^sub>L \<subseteq> \<lbrakk>\<lbrakk> \<Gamma>\<^sub>1 \<rbrakk>\<rbrakk>\<^sub>s\<^sub>y\<^sub>m\<^sub>r\<^sub>u\<^sub>n \<inter> \<lbrakk>\<lbrakk> \<Psi>\<^sub>1 \<nabla> n\<^sub>1 \<rbrakk>\<rbrakk>\<^sub>T\<^sub>E\<^sub>S\<^sub>L \<inter> \<lbrakk>\<lbrakk> \<Phi>\<^sub>1 \<nabla> Suc n\<^sub>1 \<rbrakk>\<rbrakk>\<^sub>T\<^sub>E\<^sub>S\<^sub>L"
+      using f3 a2 a1 by blast
+  qed
   show "\<And>\<Gamma> n K\<^sub>1 \<tau> K\<^sub>2 \<Psi> \<Phi>.
        (\<Gamma>\<^sub>1, n\<^sub>1 \<turnstile> \<Psi>\<^sub>1 \<triangleright> \<Phi>\<^sub>1) = (\<Gamma>, n \<turnstile> (K\<^sub>1 sporadic \<tau> on K\<^sub>2) # \<Psi> \<triangleright> \<Phi>) \<Longrightarrow>
-       (\<Gamma>\<^sub>2, n\<^sub>2 \<turnstile> \<Psi>\<^sub>2 \<triangleright> \<Phi>\<^sub>2) = (\<top>\<^sub>s\<^sub>y\<^sub>m\<^sub>r\<^sub>u\<^sub>n # \<top>\<^sub>s\<^sub>y\<^sub>m\<^sub>r\<^sub>u\<^sub>n # \<Gamma>, n \<turnstile> \<top>\<^sub>T\<^sub>E\<^sub>S\<^sub>L # \<Psi> \<triangleright> (K\<^sub>1 sporadic \<tau> on K\<^sub>2) # \<Phi>) \<Longrightarrow>
+       (\<Gamma>\<^sub>2, n\<^sub>2 \<turnstile> \<Psi>\<^sub>2 \<triangleright> \<Phi>\<^sub>2) = (\<Gamma>, n \<turnstile> \<Psi> \<triangleright> (K\<^sub>1 sporadic \<tau> on K\<^sub>2) # \<Phi>) \<Longrightarrow>
        consistent_run \<Gamma> \<Longrightarrow>
        \<lbrakk>\<lbrakk> \<Gamma>\<^sub>2 \<rbrakk>\<rbrakk>\<^sub>s\<^sub>y\<^sub>m\<^sub>r\<^sub>u\<^sub>n \<inter> \<lbrakk>\<lbrakk> \<Psi>\<^sub>2 \<nabla> n\<^sub>2 \<rbrakk>\<rbrakk>\<^sub>T\<^sub>E\<^sub>S\<^sub>L \<inter> \<lbrakk>\<lbrakk> \<Phi>\<^sub>2 \<nabla> Suc n\<^sub>2 \<rbrakk>\<rbrakk>\<^sub>T\<^sub>E\<^sub>S\<^sub>L \<subseteq> \<lbrakk>\<lbrakk> \<Gamma>\<^sub>1 \<rbrakk>\<rbrakk>\<^sub>s\<^sub>y\<^sub>m\<^sub>r\<^sub>u\<^sub>n \<inter> \<lbrakk>\<lbrakk> \<Psi>\<^sub>1 \<nabla> n\<^sub>1 \<rbrakk>\<rbrakk>\<^sub>T\<^sub>E\<^sub>S\<^sub>L \<inter> \<lbrakk>\<lbrakk> \<Phi>\<^sub>1 \<nabla> Suc n\<^sub>1 \<rbrakk>\<rbrakk>\<^sub>T\<^sub>E\<^sub>S\<^sub>L"
-    using elimination_refinement assms by fastforce
+    using TESL_interp_at_index_sporadicon_cases
+    proof -
+    fix \<Gamma> :: "constr list" and n :: nat and K\<^sub>1 :: clock and \<tau> :: tag_expr and K\<^sub>2 :: clock and \<Psi> :: "TESL_atomic list" and \<Phi> :: "TESL_atomic list"
+    assume a1: "(\<Gamma>\<^sub>1, n\<^sub>1 \<turnstile> \<Psi>\<^sub>1 \<triangleright> \<Phi>\<^sub>1) = (\<Gamma>, n \<turnstile> (K\<^sub>1 sporadic \<tau> on K\<^sub>2) # \<Psi> \<triangleright> \<Phi>)"
+    assume a2: "(\<Gamma>\<^sub>2, n\<^sub>2 \<turnstile> \<Psi>\<^sub>2 \<triangleright> \<Phi>\<^sub>2) = (\<Gamma>, n \<turnstile> \<Psi> \<triangleright> (K\<^sub>1 sporadic \<tau> on K\<^sub>2) # \<Phi>)"
+    have "n\<^sub>1 = n \<and> (\<Psi>\<^sub>1, \<Phi>\<^sub>1) = ((K\<^sub>1 sporadic \<tau> on K\<^sub>2) # \<Psi>, \<Phi>)"
+      using a1 by fastforce
+    then have f3: "\<lbrakk> K\<^sub>1 sporadic \<tau> on K\<^sub>2 \<nabla> Suc n\<^sub>1 \<rbrakk>\<^sub>T\<^sub>E\<^sub>S\<^sub>L \<subseteq> \<lbrakk> K\<^sub>1 sporadic \<tau> on K\<^sub>2 \<nabla> n \<rbrakk>\<^sub>T\<^sub>E\<^sub>S\<^sub>L"
+      using TESL_interp_at_index_sporadicon_cases by blast
+    have f4: "\<lbrakk> K\<^sub>1 sporadic \<tau> on K\<^sub>2 \<nabla> Suc n\<^sub>1 \<rbrakk>\<^sub>T\<^sub>E\<^sub>S\<^sub>L \<inter> \<lbrakk>\<lbrakk> \<Phi>\<^sub>1 \<nabla> Suc n\<^sub>1 \<rbrakk>\<rbrakk>\<^sub>T\<^sub>E\<^sub>S\<^sub>L = \<lbrakk>\<lbrakk> \<Phi>\<^sub>2 \<nabla> Suc n\<^sub>2 \<rbrakk>\<rbrakk>\<^sub>T\<^sub>E\<^sub>S\<^sub>L"
+      using a2 a1 by force
+    have "\<lbrakk> K\<^sub>1 sporadic \<tau> on K\<^sub>2 \<nabla> n \<rbrakk>\<^sub>T\<^sub>E\<^sub>S\<^sub>L \<inter> \<lbrakk>\<lbrakk> \<Psi>\<^sub>2 \<nabla> n\<^sub>2 \<rbrakk>\<rbrakk>\<^sub>T\<^sub>E\<^sub>S\<^sub>L = \<lbrakk>\<lbrakk> \<Psi>\<^sub>1 \<nabla> n\<^sub>1 \<rbrakk>\<rbrakk>\<^sub>T\<^sub>E\<^sub>S\<^sub>L"
+      using a2 a1 by force
+    then show "\<lbrakk>\<lbrakk> \<Gamma>\<^sub>2 \<rbrakk>\<rbrakk>\<^sub>s\<^sub>y\<^sub>m\<^sub>r\<^sub>u\<^sub>n \<inter> \<lbrakk>\<lbrakk> \<Psi>\<^sub>2 \<nabla> n\<^sub>2 \<rbrakk>\<rbrakk>\<^sub>T\<^sub>E\<^sub>S\<^sub>L \<inter> \<lbrakk>\<lbrakk> \<Phi>\<^sub>2 \<nabla> Suc n\<^sub>2 \<rbrakk>\<rbrakk>\<^sub>T\<^sub>E\<^sub>S\<^sub>L \<subseteq> \<lbrakk>\<lbrakk> \<Gamma>\<^sub>1 \<rbrakk>\<rbrakk>\<^sub>s\<^sub>y\<^sub>m\<^sub>r\<^sub>u\<^sub>n \<inter> \<lbrakk>\<lbrakk> \<Psi>\<^sub>1 \<nabla> n\<^sub>1 \<rbrakk>\<rbrakk>\<^sub>T\<^sub>E\<^sub>S\<^sub>L \<inter> \<lbrakk>\<lbrakk> \<Phi>\<^sub>1 \<nabla> Suc n\<^sub>1 \<rbrakk>\<rbrakk>\<^sub>T\<^sub>E\<^sub>S\<^sub>L"
+      using f4 f3 a2 a1 by blast
+  qed
   show "\<And>K\<^sub>1 n K\<^sub>2 \<tau> \<Gamma> \<Psi> \<Phi>.
        (\<Gamma>\<^sub>1, n\<^sub>1 \<turnstile> \<Psi>\<^sub>1 \<triangleright> \<Phi>\<^sub>1) = (\<Gamma>, n \<turnstile> (K\<^sub>1 sporadic \<tau> on K\<^sub>2) # \<Psi> \<triangleright> \<Phi>) \<Longrightarrow>
-       (\<Gamma>\<^sub>2, n\<^sub>2 \<turnstile> \<Psi>\<^sub>2 \<triangleright> \<Phi>\<^sub>2) = (K\<^sub>1 \<Up> n # K\<^sub>2 \<Down> n @ \<tau> # \<Gamma>, n \<turnstile> \<top>\<^sub>T\<^sub>E\<^sub>S\<^sub>L # \<Psi> \<triangleright> \<top>\<^sub>T\<^sub>E\<^sub>S\<^sub>L # \<Phi>) \<Longrightarrow>
+       (\<Gamma>\<^sub>2, n\<^sub>2 \<turnstile> \<Psi>\<^sub>2 \<triangleright> \<Phi>\<^sub>2) = (K\<^sub>1 \<Up> n # K\<^sub>2 \<Down> n @ \<tau> # \<Gamma>, n \<turnstile> \<Psi> \<triangleright> \<Phi>) \<Longrightarrow>
        consistent_run (K\<^sub>1 \<Up> n # K\<^sub>2 \<Down> n @ \<tau> # \<Gamma>) \<Longrightarrow>
        \<lbrakk>\<lbrakk> \<Gamma>\<^sub>2 \<rbrakk>\<rbrakk>\<^sub>s\<^sub>y\<^sub>m\<^sub>r\<^sub>u\<^sub>n \<inter> \<lbrakk>\<lbrakk> \<Psi>\<^sub>2 \<nabla> n\<^sub>2 \<rbrakk>\<rbrakk>\<^sub>T\<^sub>E\<^sub>S\<^sub>L \<inter> \<lbrakk>\<lbrakk> \<Phi>\<^sub>2 \<nabla> Suc n\<^sub>2 \<rbrakk>\<rbrakk>\<^sub>T\<^sub>E\<^sub>S\<^sub>L \<subseteq> \<lbrakk>\<lbrakk> \<Gamma>\<^sub>1 \<rbrakk>\<rbrakk>\<^sub>s\<^sub>y\<^sub>m\<^sub>r\<^sub>u\<^sub>n \<inter> \<lbrakk>\<lbrakk> \<Psi>\<^sub>1 \<nabla> n\<^sub>1 \<rbrakk>\<rbrakk>\<^sub>T\<^sub>E\<^sub>S\<^sub>L \<inter> \<lbrakk>\<lbrakk> \<Phi>\<^sub>1 \<nabla> Suc n\<^sub>1 \<rbrakk>\<rbrakk>\<^sub>T\<^sub>E\<^sub>S\<^sub>L"
-    using elimination_refinement assms by fastforce
+    using TESL_interp_at_index_sporadicon_cases
+    proof -
+    fix K\<^sub>1 :: clock and n :: nat and K\<^sub>2 :: clock and \<tau> :: tag_expr and \<Gamma> :: "constr list" and \<Psi> :: "TESL_atomic list" and \<Phi> :: "TESL_atomic list"
+    assume a1: "(\<Gamma>\<^sub>1, n\<^sub>1 \<turnstile> \<Psi>\<^sub>1 \<triangleright> \<Phi>\<^sub>1) = (\<Gamma>, n \<turnstile> (K\<^sub>1 sporadic \<tau> on K\<^sub>2) # \<Psi> \<triangleright> \<Phi>)"
+    assume a2: "(\<Gamma>\<^sub>2, n\<^sub>2 \<turnstile> \<Psi>\<^sub>2 \<triangleright> \<Phi>\<^sub>2) = (K\<^sub>1 \<Up> n # K\<^sub>2 \<Down> n @ \<tau> # \<Gamma>, n \<turnstile> \<Psi> \<triangleright> \<Phi>)"
+    then have f3: "\<lbrakk>\<lbrakk> \<Gamma>\<^sub>1 \<rbrakk>\<rbrakk>\<^sub>s\<^sub>y\<^sub>m\<^sub>r\<^sub>u\<^sub>n \<inter> (\<lbrakk>\<lbrakk> \<Gamma>\<^sub>2 \<rbrakk>\<rbrakk>\<^sub>s\<^sub>y\<^sub>m\<^sub>r\<^sub>u\<^sub>n \<inter> (\<lbrakk>\<lbrakk> \<Psi>\<^sub>2 \<nabla> n\<^sub>2 \<rbrakk>\<rbrakk>\<^sub>T\<^sub>E\<^sub>S\<^sub>L \<inter> \<lbrakk>\<lbrakk> \<Phi>\<^sub>2 \<nabla> Suc n\<^sub>2 \<rbrakk>\<rbrakk>\<^sub>T\<^sub>E\<^sub>S\<^sub>L)) \<subseteq> (\<Inter>t\<in>set \<Psi>\<^sub>2. \<lbrakk> t \<nabla> n\<^sub>2 \<rbrakk>\<^sub>T\<^sub>E\<^sub>S\<^sub>L) \<inter> (\<lbrakk>\<lbrakk> \<Gamma>\<^sub>1 \<rbrakk>\<rbrakk>\<^sub>s\<^sub>y\<^sub>m\<^sub>r\<^sub>u\<^sub>n \<inter> (\<Inter>t\<in>set \<Phi>\<^sub>1. \<lbrakk> t \<nabla> Suc n\<^sub>1 \<rbrakk>\<^sub>T\<^sub>E\<^sub>S\<^sub>L))"
+    using a1 TESL_interpretation_at_index_fixpoint by force
+    have f4: "\<lbrakk> K\<^sub>1 \<Up> n \<rbrakk>\<^sub>s\<^sub>y\<^sub>m\<^sub>r\<^sub>u\<^sub>n \<inter> (\<lbrakk> K\<^sub>2 \<Down> n @ \<tau> \<rbrakk>\<^sub>s\<^sub>y\<^sub>m\<^sub>r\<^sub>u\<^sub>n \<inter> \<lbrakk> K\<^sub>2 \<Down> n @ \<tau> \<rbrakk>\<^sub>s\<^sub>y\<^sub>m\<^sub>r\<^sub>u\<^sub>n) \<inter> (\<lbrakk>\<lbrakk> \<Gamma>\<^sub>1 \<rbrakk>\<rbrakk>\<^sub>s\<^sub>y\<^sub>m\<^sub>r\<^sub>u\<^sub>n \<inter> (\<lbrakk>\<lbrakk> \<Gamma>\<^sub>2 \<rbrakk>\<rbrakk>\<^sub>s\<^sub>y\<^sub>m\<^sub>r\<^sub>u\<^sub>n \<inter> (\<lbrakk>\<lbrakk> \<Psi>\<^sub>2 \<nabla> n\<^sub>2 \<rbrakk>\<rbrakk>\<^sub>T\<^sub>E\<^sub>S\<^sub>L \<inter> \<lbrakk>\<lbrakk> \<Phi>\<^sub>2 \<nabla> Suc n\<^sub>2 \<rbrakk>\<rbrakk>\<^sub>T\<^sub>E\<^sub>S\<^sub>L))) = \<lbrakk>\<lbrakk> \<Gamma>\<^sub>2 \<rbrakk>\<rbrakk>\<^sub>s\<^sub>y\<^sub>m\<^sub>r\<^sub>u\<^sub>n \<inter> (\<lbrakk>\<lbrakk> \<Psi>\<^sub>2 \<nabla> n\<^sub>2 \<rbrakk>\<rbrakk>\<^sub>T\<^sub>E\<^sub>S\<^sub>L \<inter> \<lbrakk>\<lbrakk> \<Phi>\<^sub>2 \<nabla> Suc n\<^sub>2 \<rbrakk>\<rbrakk>\<^sub>T\<^sub>E\<^sub>S\<^sub>L)"
+      using a2 a1 by force
+    have "\<lbrakk> K\<^sub>1 sporadic \<tau> on K\<^sub>2 \<nabla> n \<rbrakk>\<^sub>T\<^sub>E\<^sub>S\<^sub>L \<inter> (\<Inter>t\<in>set \<Psi>\<^sub>2. \<lbrakk> t \<nabla> n\<^sub>2 \<rbrakk>\<^sub>T\<^sub>E\<^sub>S\<^sub>L) \<inter> (\<lbrakk>\<lbrakk> \<Gamma>\<^sub>1 \<rbrakk>\<rbrakk>\<^sub>s\<^sub>y\<^sub>m\<^sub>r\<^sub>u\<^sub>n \<inter> (\<Inter>t\<in>set \<Phi>\<^sub>1. \<lbrakk> t \<nabla> Suc n\<^sub>1 \<rbrakk>\<^sub>T\<^sub>E\<^sub>S\<^sub>L)) = (\<Inter>t\<in>set \<Psi>\<^sub>1. \<lbrakk> t \<nabla> n\<^sub>1 \<rbrakk>\<^sub>T\<^sub>E\<^sub>S\<^sub>L) \<inter> (\<lbrakk>\<lbrakk> \<Gamma>\<^sub>1 \<rbrakk>\<rbrakk>\<^sub>s\<^sub>y\<^sub>m\<^sub>r\<^sub>u\<^sub>n \<inter> (\<lbrakk>\<lbrakk> \<Gamma>\<^sub>1 \<rbrakk>\<rbrakk>\<^sub>s\<^sub>y\<^sub>m\<^sub>r\<^sub>u\<^sub>n \<inter> (\<Inter>t\<in>set \<Phi>\<^sub>1. \<lbrakk> t \<nabla> Suc n\<^sub>1 \<rbrakk>\<^sub>T\<^sub>E\<^sub>S\<^sub>L)))"
+      using a2 a1 by simp
+    then have "(\<lbrakk> K\<^sub>1 \<Up> n \<rbrakk>\<^sub>s\<^sub>y\<^sub>m\<^sub>r\<^sub>u\<^sub>n \<inter> \<lbrakk> K\<^sub>2 \<Down> n @ \<tau> \<rbrakk>\<^sub>s\<^sub>y\<^sub>m\<^sub>r\<^sub>u\<^sub>n \<union> \<lbrakk> K\<^sub>1 sporadic \<tau> on K\<^sub>2 \<nabla> Suc n \<rbrakk>\<^sub>T\<^sub>E\<^sub>S\<^sub>L) \<inter> ((\<Inter>t\<in>set \<Psi>\<^sub>2. \<lbrakk> t \<nabla> n\<^sub>2 \<rbrakk>\<^sub>T\<^sub>E\<^sub>S\<^sub>L) \<inter> (\<lbrakk>\<lbrakk> \<Gamma>\<^sub>1 \<rbrakk>\<rbrakk>\<^sub>s\<^sub>y\<^sub>m\<^sub>r\<^sub>u\<^sub>n \<inter> (\<Inter>t\<in>set \<Phi>\<^sub>1. \<lbrakk> t \<nabla> Suc n\<^sub>1 \<rbrakk>\<^sub>T\<^sub>E\<^sub>S\<^sub>L))) = \<lbrakk>\<lbrakk> \<Gamma>\<^sub>1 \<rbrakk>\<rbrakk>\<^sub>s\<^sub>y\<^sub>m\<^sub>r\<^sub>u\<^sub>n \<inter> (\<lbrakk>\<lbrakk> \<Psi>\<^sub>1 \<nabla> n\<^sub>1 \<rbrakk>\<rbrakk>\<^sub>T\<^sub>E\<^sub>S\<^sub>L \<inter> \<lbrakk>\<lbrakk> \<Phi>\<^sub>1 \<nabla> Suc n\<^sub>1 \<rbrakk>\<rbrakk>\<^sub>T\<^sub>E\<^sub>S\<^sub>L)"
+      by (metis Int_absorb TESL_interp_at_index_sporadicon_cases TESL_interpretation_at_index_fixpoint inf_aci(2) inf_left_commute)
+    then show "\<lbrakk>\<lbrakk> \<Gamma>\<^sub>2 \<rbrakk>\<rbrakk>\<^sub>s\<^sub>y\<^sub>m\<^sub>r\<^sub>u\<^sub>n \<inter> \<lbrakk>\<lbrakk> \<Psi>\<^sub>2 \<nabla> n\<^sub>2 \<rbrakk>\<rbrakk>\<^sub>T\<^sub>E\<^sub>S\<^sub>L \<inter> \<lbrakk>\<lbrakk> \<Phi>\<^sub>2 \<nabla> Suc n\<^sub>2 \<rbrakk>\<rbrakk>\<^sub>T\<^sub>E\<^sub>S\<^sub>L \<subseteq> \<lbrakk>\<lbrakk> \<Gamma>\<^sub>1 \<rbrakk>\<rbrakk>\<^sub>s\<^sub>y\<^sub>m\<^sub>r\<^sub>u\<^sub>n \<inter> \<lbrakk>\<lbrakk> \<Psi>\<^sub>1 \<nabla> n\<^sub>1 \<rbrakk>\<rbrakk>\<^sub>T\<^sub>E\<^sub>S\<^sub>L \<inter> \<lbrakk>\<lbrakk> \<Phi>\<^sub>1 \<nabla> Suc n\<^sub>1 \<rbrakk>\<rbrakk>\<^sub>T\<^sub>E\<^sub>S\<^sub>L"
+      using f4 f3 by blast
+  qed
   show "\<And>K\<^sub>1 n \<alpha> K\<^sub>2 \<beta> \<Gamma> \<Psi> \<Phi>.
        (\<Gamma>\<^sub>1, n\<^sub>1 \<turnstile> \<Psi>\<^sub>1 \<triangleright> \<Phi>\<^sub>1) = (\<Gamma>, n \<turnstile> (tag-relation K\<^sub>1 = \<alpha> * K\<^sub>2 + \<beta>) # \<Psi> \<triangleright> \<Phi>) \<Longrightarrow>
-       (\<Gamma>\<^sub>2, n\<^sub>2 \<turnstile> \<Psi>\<^sub>2 \<triangleright> \<Phi>\<^sub>2) = (\<top>\<^sub>s\<^sub>y\<^sub>m\<^sub>r\<^sub>u\<^sub>n # \<tau>\<^sub>v\<^sub>a\<^sub>r (K\<^sub>1, n) \<doteq> \<alpha> * \<tau>\<^sub>v\<^sub>a\<^sub>r (K\<^sub>2, n) + \<beta> # \<Gamma>, n \<turnstile> \<top>\<^sub>T\<^sub>E\<^sub>S\<^sub>L # \<Psi> \<triangleright> (tag-relation K\<^sub>1 = \<alpha> * K\<^sub>2 + \<beta>) # \<Phi>) \<Longrightarrow>
+       (\<Gamma>\<^sub>2, n\<^sub>2 \<turnstile> \<Psi>\<^sub>2 \<triangleright> \<Phi>\<^sub>2) = (\<tau>\<^sub>v\<^sub>a\<^sub>r (K\<^sub>1, n) \<doteq> \<alpha> * \<tau>\<^sub>v\<^sub>a\<^sub>r (K\<^sub>2, n) + \<beta> # \<Gamma>, n \<turnstile> \<Psi> \<triangleright> (tag-relation K\<^sub>1 = \<alpha> * K\<^sub>2 + \<beta>) # \<Phi>) \<Longrightarrow>
        consistent_run (\<tau>\<^sub>v\<^sub>a\<^sub>r (K\<^sub>1, n) \<doteq> \<alpha> * \<tau>\<^sub>v\<^sub>a\<^sub>r (K\<^sub>2, n) + \<beta> # \<Gamma>) \<Longrightarrow>
        \<lbrakk>\<lbrakk> \<Gamma>\<^sub>2 \<rbrakk>\<rbrakk>\<^sub>s\<^sub>y\<^sub>m\<^sub>r\<^sub>u\<^sub>n \<inter> \<lbrakk>\<lbrakk> \<Psi>\<^sub>2 \<nabla> n\<^sub>2 \<rbrakk>\<rbrakk>\<^sub>T\<^sub>E\<^sub>S\<^sub>L \<inter> \<lbrakk>\<lbrakk> \<Phi>\<^sub>2 \<nabla> Suc n\<^sub>2 \<rbrakk>\<rbrakk>\<^sub>T\<^sub>E\<^sub>S\<^sub>L \<subseteq> \<lbrakk>\<lbrakk> \<Gamma>\<^sub>1 \<rbrakk>\<rbrakk>\<^sub>s\<^sub>y\<^sub>m\<^sub>r\<^sub>u\<^sub>n \<inter> \<lbrakk>\<lbrakk> \<Psi>\<^sub>1 \<nabla> n\<^sub>1 \<rbrakk>\<rbrakk>\<^sub>T\<^sub>E\<^sub>S\<^sub>L \<inter> \<lbrakk>\<lbrakk> \<Phi>\<^sub>1 \<nabla> Suc n\<^sub>1 \<rbrakk>\<rbrakk>\<^sub>T\<^sub>E\<^sub>S\<^sub>L"
-    using elimination_refinement
-    by (metis (no_types, lifting) Pair_inject TESL_interpretation_at_index_cons_morph assms inf_sup_aci(2) symbolic_run_interpretation.simps(2))
+    using TESL_interp_at_index_tagrel_cases
+    proof -
+      fix K\<^sub>1 :: clock and n :: nat and \<alpha> :: tag_const and K\<^sub>2 :: clock and \<beta> :: tag_const and \<Gamma> :: "constr list" and \<Psi> :: "TESL_atomic list" and \<Phi> :: "TESL_atomic list"
+    assume a1: "(\<Gamma>\<^sub>2, n\<^sub>2 \<turnstile> \<Psi>\<^sub>2 \<triangleright> \<Phi>\<^sub>2) = (\<tau>\<^sub>v\<^sub>a\<^sub>r (K\<^sub>1, n) \<doteq> \<alpha> * \<tau>\<^sub>v\<^sub>a\<^sub>r (K\<^sub>2, n) + \<beta> # \<Gamma>, n \<turnstile> \<Psi> \<triangleright> (tag-relation K\<^sub>1 = \<alpha> * K\<^sub>2 + \<beta>) # \<Phi>)"
+    assume a2: "(\<Gamma>\<^sub>1, n\<^sub>1 \<turnstile> \<Psi>\<^sub>1 \<triangleright> \<Phi>\<^sub>1) = (\<Gamma>, n \<turnstile> (tag-relation K\<^sub>1 = \<alpha> * K\<^sub>2 + \<beta>) # \<Psi> \<triangleright> \<Phi>)"
+    have f3: "\<forall>ts tsa tsb tsc. (ts::TESL_atomic list, tsa::TESL_atomic list) \<noteq> (tsb, tsc) \<or> ts = tsb \<and> tsa = tsc"
+      by fastforce
+    have f4: "n\<^sub>2 = n \<and> (\<Psi>\<^sub>2, \<Phi>\<^sub>2) = (\<Psi>, (tag-relation K\<^sub>1 = \<alpha> * K\<^sub>2 + \<beta>) # \<Phi>)"
+      using a1 by fastforce
+    have f5: "\<lbrakk>\<lbrakk> (tag-relation K\<^sub>1 = \<alpha> * K\<^sub>2 + \<beta>) # \<Phi> \<nabla> Suc n \<rbrakk>\<rbrakk>\<^sub>T\<^sub>E\<^sub>S\<^sub>L = \<lbrakk>\<lbrakk> \<Phi>\<^sub>2 \<nabla> Suc n\<^sub>2 \<rbrakk>\<rbrakk>\<^sub>T\<^sub>E\<^sub>S\<^sub>L"
+      using a1 by force
+    have f6: "n\<^sub>1 = n \<and> (\<Psi>\<^sub>1, \<Phi>\<^sub>1) = ((tag-relation K\<^sub>1 = \<alpha> * K\<^sub>2 + \<beta>) # \<Psi>, \<Phi>)"
+      using a2 by fastforce
+    have f7: "\<lbrakk>\<lbrakk> \<Phi> \<nabla> Suc n \<rbrakk>\<rbrakk>\<^sub>T\<^sub>E\<^sub>S\<^sub>L = \<lbrakk>\<lbrakk> \<Phi>\<^sub>1 \<nabla> Suc n\<^sub>1 \<rbrakk>\<rbrakk>\<^sub>T\<^sub>E\<^sub>S\<^sub>L"
+      using a2 by force
+    have f8: "\<lbrakk>\<lbrakk> \<tau>\<^sub>v\<^sub>a\<^sub>r (K\<^sub>1, n) \<doteq> \<alpha> * \<tau>\<^sub>v\<^sub>a\<^sub>r (K\<^sub>2, n) + \<beta> # \<Gamma> \<rbrakk>\<rbrakk>\<^sub>s\<^sub>y\<^sub>m\<^sub>r\<^sub>u\<^sub>n = \<lbrakk> \<tau>\<^sub>v\<^sub>a\<^sub>r (K\<^sub>1, n) \<doteq> \<alpha> * \<tau>\<^sub>v\<^sub>a\<^sub>r (K\<^sub>2, n) + \<beta> \<rbrakk>\<^sub>s\<^sub>y\<^sub>m\<^sub>r\<^sub>u\<^sub>n \<inter> \<lbrakk>\<lbrakk> \<Gamma>\<^sub>1 \<rbrakk>\<rbrakk>\<^sub>s\<^sub>y\<^sub>m\<^sub>r\<^sub>u\<^sub>n"
+      using a2 by force
+    have f9: "\<lbrakk> tag-relation K\<^sub>1 = \<alpha> * K\<^sub>2 + \<beta> \<nabla> Suc n \<rbrakk>\<^sub>T\<^sub>E\<^sub>S\<^sub>L \<inter> (\<lbrakk>\<lbrakk> \<Psi>\<^sub>2 \<nabla> n\<^sub>2 \<rbrakk>\<rbrakk>\<^sub>T\<^sub>E\<^sub>S\<^sub>L \<inter> \<lbrakk> \<tau>\<^sub>v\<^sub>a\<^sub>r (K\<^sub>1, n) \<doteq> \<alpha> * \<tau>\<^sub>v\<^sub>a\<^sub>r (K\<^sub>2, n) + \<beta> \<rbrakk>\<^sub>s\<^sub>y\<^sub>m\<^sub>r\<^sub>u\<^sub>n) = \<lbrakk>\<lbrakk> \<Psi>\<^sub>1 \<nabla> n\<^sub>1 \<rbrakk>\<rbrakk>\<^sub>T\<^sub>E\<^sub>S\<^sub>L"
+      using f6 f4 f3 by (metis Int_commute TESL_interp_at_index_tagrel_cases TESL_interpretation_at_index_cons_morph inf_sup_aci(3))
+    have "\<lbrakk> tag-relation K\<^sub>1 = \<alpha> * K\<^sub>2 + \<beta> \<nabla> Suc n \<rbrakk>\<^sub>T\<^sub>E\<^sub>S\<^sub>L \<inter> \<lbrakk>\<lbrakk> \<Phi>\<^sub>1 \<nabla> Suc n\<^sub>1 \<rbrakk>\<rbrakk>\<^sub>T\<^sub>E\<^sub>S\<^sub>L = \<lbrakk>\<lbrakk> \<Phi>\<^sub>2 \<nabla> Suc n\<^sub>2 \<rbrakk>\<rbrakk>\<^sub>T\<^sub>E\<^sub>S\<^sub>L"
+      using f7 f5 by simp
+    then show "\<lbrakk>\<lbrakk> \<Gamma>\<^sub>2 \<rbrakk>\<rbrakk>\<^sub>s\<^sub>y\<^sub>m\<^sub>r\<^sub>u\<^sub>n \<inter> \<lbrakk>\<lbrakk> \<Psi>\<^sub>2 \<nabla> n\<^sub>2 \<rbrakk>\<rbrakk>\<^sub>T\<^sub>E\<^sub>S\<^sub>L \<inter> \<lbrakk>\<lbrakk> \<Phi>\<^sub>2 \<nabla> Suc n\<^sub>2 \<rbrakk>\<rbrakk>\<^sub>T\<^sub>E\<^sub>S\<^sub>L \<subseteq> \<lbrakk>\<lbrakk> \<Gamma>\<^sub>1 \<rbrakk>\<rbrakk>\<^sub>s\<^sub>y\<^sub>m\<^sub>r\<^sub>u\<^sub>n \<inter> \<lbrakk>\<lbrakk> \<Psi>\<^sub>1 \<nabla> n\<^sub>1 \<rbrakk>\<rbrakk>\<^sub>T\<^sub>E\<^sub>S\<^sub>L \<inter> \<lbrakk>\<lbrakk> \<Phi>\<^sub>1 \<nabla> Suc n\<^sub>1 \<rbrakk>\<rbrakk>\<^sub>T\<^sub>E\<^sub>S\<^sub>L"
+      using f9 f8 a1 by blast
+  qed
   show "\<And>K\<^sub>1 n \<Gamma> K\<^sub>2 \<Psi> \<Phi>.
        (\<Gamma>\<^sub>1, n\<^sub>1 \<turnstile> \<Psi>\<^sub>1 \<triangleright> \<Phi>\<^sub>1) = (\<Gamma>, n \<turnstile> (K\<^sub>1 implies K\<^sub>2) # \<Psi> \<triangleright> \<Phi>) \<Longrightarrow>
-       (\<Gamma>\<^sub>2, n\<^sub>2 \<turnstile> \<Psi>\<^sub>2 \<triangleright> \<Phi>\<^sub>2) = (\<top>\<^sub>s\<^sub>y\<^sub>m\<^sub>r\<^sub>u\<^sub>n # K\<^sub>1 \<not>\<Up> n # \<Gamma>, n \<turnstile> \<top>\<^sub>T\<^sub>E\<^sub>S\<^sub>L # \<Psi> \<triangleright> (K\<^sub>1 implies K\<^sub>2) # \<Phi>) \<Longrightarrow>
+       (\<Gamma>\<^sub>2, n\<^sub>2 \<turnstile> \<Psi>\<^sub>2 \<triangleright> \<Phi>\<^sub>2) = (K\<^sub>1 \<not>\<Up> n # \<Gamma>, n \<turnstile> \<Psi> \<triangleright> (K\<^sub>1 implies K\<^sub>2) # \<Phi>) \<Longrightarrow>
        consistent_run (K\<^sub>1 \<not>\<Up> n # \<Gamma>) \<Longrightarrow>
        \<lbrakk>\<lbrakk> \<Gamma>\<^sub>2 \<rbrakk>\<rbrakk>\<^sub>s\<^sub>y\<^sub>m\<^sub>r\<^sub>u\<^sub>n \<inter> \<lbrakk>\<lbrakk> \<Psi>\<^sub>2 \<nabla> n\<^sub>2 \<rbrakk>\<rbrakk>\<^sub>T\<^sub>E\<^sub>S\<^sub>L \<inter> \<lbrakk>\<lbrakk> \<Phi>\<^sub>2 \<nabla> Suc n\<^sub>2 \<rbrakk>\<rbrakk>\<^sub>T\<^sub>E\<^sub>S\<^sub>L \<subseteq> \<lbrakk>\<lbrakk> \<Gamma>\<^sub>1 \<rbrakk>\<rbrakk>\<^sub>s\<^sub>y\<^sub>m\<^sub>r\<^sub>u\<^sub>n \<inter> \<lbrakk>\<lbrakk> \<Psi>\<^sub>1 \<nabla> n\<^sub>1 \<rbrakk>\<rbrakk>\<^sub>T\<^sub>E\<^sub>S\<^sub>L \<inter> \<lbrakk>\<lbrakk> \<Phi>\<^sub>1 \<nabla> Suc n\<^sub>1 \<rbrakk>\<rbrakk>\<^sub>T\<^sub>E\<^sub>S\<^sub>L"
-    using elimination_refinement
-    by (metis (no_types, lifting) Pair_inject TESL_interpretation_at_index_cons_morph assms inf.assoc symbolic_run_interpretation.simps(2))
+    using TESL_interp_at_index_implies_cases
+    using [[smt_solver = cvc4]]
+    by (smt Int_subset_iff Pair_inject TESL_interpretation_at_index.elims inf.cobounded2 inf.mono inf_sup_aci(2) list.simps(1) list.simps(3) sup.cobounded1 symbolic_run_interpretation.simps(2))
   show "\<And>K\<^sub>1 n K\<^sub>2 \<Gamma> \<Psi> \<Phi>.
        (\<Gamma>\<^sub>1, n\<^sub>1 \<turnstile> \<Psi>\<^sub>1 \<triangleright> \<Phi>\<^sub>1) = (\<Gamma>, n \<turnstile> (K\<^sub>1 implies K\<^sub>2) # \<Psi> \<triangleright> \<Phi>) \<Longrightarrow>
-       (\<Gamma>\<^sub>2, n\<^sub>2 \<turnstile> \<Psi>\<^sub>2 \<triangleright> \<Phi>\<^sub>2) = (K\<^sub>1 \<Up> n # K\<^sub>2 \<Up> n # \<Gamma>, n \<turnstile> \<top>\<^sub>T\<^sub>E\<^sub>S\<^sub>L # \<Psi> \<triangleright> (K\<^sub>1 implies K\<^sub>2) # \<Phi>) \<Longrightarrow>
+       (\<Gamma>\<^sub>2, n\<^sub>2 \<turnstile> \<Psi>\<^sub>2 \<triangleright> \<Phi>\<^sub>2) = (K\<^sub>1 \<Up> n # K\<^sub>2 \<Up> n # \<Gamma>, n \<turnstile> \<Psi> \<triangleright> (K\<^sub>1 implies K\<^sub>2) # \<Phi>) \<Longrightarrow>
        consistent_run (K\<^sub>1 \<Up> n # K\<^sub>2 \<Up> n # \<Gamma>) \<Longrightarrow>
        \<lbrakk>\<lbrakk> \<Gamma>\<^sub>2 \<rbrakk>\<rbrakk>\<^sub>s\<^sub>y\<^sub>m\<^sub>r\<^sub>u\<^sub>n \<inter> \<lbrakk>\<lbrakk> \<Psi>\<^sub>2 \<nabla> n\<^sub>2 \<rbrakk>\<rbrakk>\<^sub>T\<^sub>E\<^sub>S\<^sub>L \<inter> \<lbrakk>\<lbrakk> \<Phi>\<^sub>2 \<nabla> Suc n\<^sub>2 \<rbrakk>\<rbrakk>\<^sub>T\<^sub>E\<^sub>S\<^sub>L \<subseteq> \<lbrakk>\<lbrakk> \<Gamma>\<^sub>1 \<rbrakk>\<rbrakk>\<^sub>s\<^sub>y\<^sub>m\<^sub>r\<^sub>u\<^sub>n \<inter> \<lbrakk>\<lbrakk> \<Psi>\<^sub>1 \<nabla> n\<^sub>1 \<rbrakk>\<rbrakk>\<^sub>T\<^sub>E\<^sub>S\<^sub>L \<inter> \<lbrakk>\<lbrakk> \<Phi>\<^sub>1 \<nabla> Suc n\<^sub>1 \<rbrakk>\<rbrakk>\<^sub>T\<^sub>E\<^sub>S\<^sub>L"
-    using elimination_refinement
-    by (metis (no_types, lifting) Pair_inject TESL_interpretation_at_index_cons_morph assms inf_assoc symbolic_run_interpretation.simps(2))
+    using TESL_interp_at_index_implies_cases
+    using [[smt_solver = cvc4]]
+    by (smt Int_subset_iff Pair_inject TESL_interpretation_at_index_cons_morph inf_le1 inf_sup_aci(2) le_iff_inf sup.cobounded2 symbolic_run_interpretation.simps(2))
   show "\<And>K\<^sub>1 n \<Gamma> \<delta>\<tau> K\<^sub>2 K\<^sub>3 \<Psi> \<Phi>.
        (\<Gamma>\<^sub>1, n\<^sub>1 \<turnstile> \<Psi>\<^sub>1 \<triangleright> \<Phi>\<^sub>1) = (\<Gamma>, n \<turnstile> (K\<^sub>1 time-delayed by \<delta>\<tau> on K\<^sub>2 implies K\<^sub>3) # \<Psi> \<triangleright> \<Phi>) \<Longrightarrow>
-       (\<Gamma>\<^sub>2, n\<^sub>2 \<turnstile> \<Psi>\<^sub>2 \<triangleright> \<Phi>\<^sub>2) = (\<top>\<^sub>s\<^sub>y\<^sub>m\<^sub>r\<^sub>u\<^sub>n # K\<^sub>1 \<not>\<Up> n # \<Gamma>, n \<turnstile> \<top>\<^sub>T\<^sub>E\<^sub>S\<^sub>L # \<Psi> \<triangleright> (K\<^sub>1 time-delayed by \<delta>\<tau> on K\<^sub>2 implies K\<^sub>3) # \<Phi>) \<Longrightarrow>
+       (\<Gamma>\<^sub>2, n\<^sub>2 \<turnstile> \<Psi>\<^sub>2 \<triangleright> \<Phi>\<^sub>2) = (K\<^sub>1 \<not>\<Up> n # \<Gamma>, n \<turnstile> \<Psi> \<triangleright> (K\<^sub>1 time-delayed by \<delta>\<tau> on K\<^sub>2 implies K\<^sub>3) # \<Phi>) \<Longrightarrow>
        consistent_run (K\<^sub>1 \<not>\<Up> n # \<Gamma>) \<Longrightarrow>
        \<lbrakk>\<lbrakk> \<Gamma>\<^sub>2 \<rbrakk>\<rbrakk>\<^sub>s\<^sub>y\<^sub>m\<^sub>r\<^sub>u\<^sub>n \<inter> \<lbrakk>\<lbrakk> \<Psi>\<^sub>2 \<nabla> n\<^sub>2 \<rbrakk>\<rbrakk>\<^sub>T\<^sub>E\<^sub>S\<^sub>L \<inter> \<lbrakk>\<lbrakk> \<Phi>\<^sub>2 \<nabla> Suc n\<^sub>2 \<rbrakk>\<rbrakk>\<^sub>T\<^sub>E\<^sub>S\<^sub>L \<subseteq> \<lbrakk>\<lbrakk> \<Gamma>\<^sub>1 \<rbrakk>\<rbrakk>\<^sub>s\<^sub>y\<^sub>m\<^sub>r\<^sub>u\<^sub>n \<inter> \<lbrakk>\<lbrakk> \<Psi>\<^sub>1 \<nabla> n\<^sub>1 \<rbrakk>\<rbrakk>\<^sub>T\<^sub>E\<^sub>S\<^sub>L \<inter> \<lbrakk>\<lbrakk> \<Phi>\<^sub>1 \<nabla> Suc n\<^sub>1 \<rbrakk>\<rbrakk>\<^sub>T\<^sub>E\<^sub>S\<^sub>L"
-    using elimination_refinement
-    by (metis (no_types, lifting) Int_assoc Pair_inject TESL_interpretation_at_index_cons_morph assms symbolic_run_interpretation.simps(2))
+    using TESL_interp_at_index_timedelayed_cases
+    using [[smt_solver = cvc4]]
+    by (smt Int_subset_iff Pair_inject TESL_interpretation_at_index_cons_morph inf.cobounded2 inf_le1 subset_trans sup.cobounded1 symbolic_run_interpretation.simps(2))
   show "\<And>K\<^sub>1 n \<Gamma> \<delta>\<tau> K\<^sub>2 K\<^sub>3 \<Psi> \<Phi>.
        (\<Gamma>\<^sub>1, n\<^sub>1 \<turnstile> \<Psi>\<^sub>1 \<triangleright> \<Phi>\<^sub>1) = (\<Gamma>, n \<turnstile> (K\<^sub>1 time-delayed by \<delta>\<tau> on K\<^sub>2 implies K\<^sub>3) # \<Psi> \<triangleright> \<Phi>) \<Longrightarrow>
-       (\<Gamma>\<^sub>2, n\<^sub>2 \<turnstile> \<Psi>\<^sub>2 \<triangleright> \<Phi>\<^sub>2) = (\<top>\<^sub>s\<^sub>y\<^sub>m\<^sub>r\<^sub>u\<^sub>n # K\<^sub>1 \<Up> n # \<Gamma>, n \<turnstile> (K\<^sub>3 sporadic \<lfloor> \<tau>\<^sub>v\<^sub>a\<^sub>r (K\<^sub>2, n) \<oplus> \<delta>\<tau> \<rfloor> on K\<^sub>2) # \<Psi> \<triangleright> (K\<^sub>1 time-delayed by \<delta>\<tau> on K\<^sub>2 implies K\<^sub>3) # \<Phi>) \<Longrightarrow>
+       (\<Gamma>\<^sub>2, n\<^sub>2 \<turnstile> \<Psi>\<^sub>2 \<triangleright> \<Phi>\<^sub>2) = (K\<^sub>1 \<Up> n # \<Gamma>, n \<turnstile> (K\<^sub>3 sporadic \<lfloor> \<tau>\<^sub>v\<^sub>a\<^sub>r (K\<^sub>2, n) \<oplus> \<delta>\<tau> \<rfloor> on K\<^sub>2) # \<Psi> \<triangleright> (K\<^sub>1 time-delayed by \<delta>\<tau> on K\<^sub>2 implies K\<^sub>3) # \<Phi>) \<Longrightarrow>
        consistent_run (K\<^sub>1 \<Up> n # \<Gamma>) \<Longrightarrow>
        \<lbrakk>\<lbrakk> \<Gamma>\<^sub>2 \<rbrakk>\<rbrakk>\<^sub>s\<^sub>y\<^sub>m\<^sub>r\<^sub>u\<^sub>n \<inter> \<lbrakk>\<lbrakk> \<Psi>\<^sub>2 \<nabla> n\<^sub>2 \<rbrakk>\<rbrakk>\<^sub>T\<^sub>E\<^sub>S\<^sub>L \<inter> \<lbrakk>\<lbrakk> \<Phi>\<^sub>2 \<nabla> Suc n\<^sub>2 \<rbrakk>\<rbrakk>\<^sub>T\<^sub>E\<^sub>S\<^sub>L \<subseteq> \<lbrakk>\<lbrakk> \<Gamma>\<^sub>1 \<rbrakk>\<rbrakk>\<^sub>s\<^sub>y\<^sub>m\<^sub>r\<^sub>u\<^sub>n \<inter> \<lbrakk>\<lbrakk> \<Psi>\<^sub>1 \<nabla> n\<^sub>1 \<rbrakk>\<rbrakk>\<^sub>T\<^sub>E\<^sub>S\<^sub>L \<inter> \<lbrakk>\<lbrakk> \<Phi>\<^sub>1 \<nabla> Suc n\<^sub>1 \<rbrakk>\<rbrakk>\<^sub>T\<^sub>E\<^sub>S\<^sub>L"
-    using elimination_refinement
-    by (metis (no_types, lifting) Pair_inject TESL_interpretation_at_index_cons_morph assms inf.assoc symbolic_run_interpretation.simps(2))
+    proof -
+    fix K\<^sub>1 :: clock and n :: nat and \<Gamma> :: "constr list" and \<delta>\<tau> :: tag_const and K\<^sub>2 :: clock and K\<^sub>3 :: clock and \<Psi> :: TESL_formula and \<Phi> :: TESL_formula
+    assume a1: "(\<Gamma>\<^sub>1, n\<^sub>1 \<turnstile> \<Psi>\<^sub>1 \<triangleright> \<Phi>\<^sub>1) = (\<Gamma>, n \<turnstile> (K\<^sub>1 time-delayed by \<delta>\<tau> on K\<^sub>2 implies K\<^sub>3) # \<Psi> \<triangleright> \<Phi>)"
+    assume a2: "(\<Gamma>\<^sub>2, n\<^sub>2 \<turnstile> \<Psi>\<^sub>2 \<triangleright> \<Phi>\<^sub>2) = (K\<^sub>1 \<Up> n # \<Gamma>, n \<turnstile> (K\<^sub>3 sporadic \<lfloor> \<tau>\<^sub>v\<^sub>a\<^sub>r (K\<^sub>2, n) \<oplus> \<delta>\<tau> \<rfloor> on K\<^sub>2) # \<Psi> \<triangleright> (K\<^sub>1 time-delayed by \<delta>\<tau> on K\<^sub>2 implies K\<^sub>3) # \<Phi>)"
+    have tdby_cases_corrollary: "\<lbrakk> K\<^sub>1 time-delayed by \<delta>\<tau> on K\<^sub>2 implies K\<^sub>3 \<nabla> n \<rbrakk>\<^sub>T\<^sub>E\<^sub>S\<^sub>L \<supseteq>
+        \<lbrakk> K\<^sub>1 \<Up> n \<rbrakk>\<^sub>s\<^sub>y\<^sub>m\<^sub>r\<^sub>u\<^sub>n \<inter> \<lbrakk> K\<^sub>3 sporadic \<lfloor>\<tau>\<^sub>v\<^sub>a\<^sub>r(K\<^sub>2, n) \<oplus> \<delta>\<tau>\<rfloor> on K\<^sub>2 \<nabla> n \<rbrakk>\<^sub>T\<^sub>E\<^sub>S\<^sub>L \<inter> \<lbrakk> K\<^sub>1 time-delayed by \<delta>\<tau> on K\<^sub>2 implies K\<^sub>3 \<nabla> Suc n \<rbrakk>\<^sub>T\<^sub>E\<^sub>S\<^sub>L"
+      using TESL_interp_at_index_timedelayed_cases by blast
+    then show "\<lbrakk>\<lbrakk> \<Gamma>\<^sub>2 \<rbrakk>\<rbrakk>\<^sub>s\<^sub>y\<^sub>m\<^sub>r\<^sub>u\<^sub>n \<inter> \<lbrakk>\<lbrakk> \<Psi>\<^sub>2 \<nabla> n\<^sub>2 \<rbrakk>\<rbrakk>\<^sub>T\<^sub>E\<^sub>S\<^sub>L \<inter> \<lbrakk>\<lbrakk> \<Phi>\<^sub>2 \<nabla> Suc n\<^sub>2 \<rbrakk>\<rbrakk>\<^sub>T\<^sub>E\<^sub>S\<^sub>L \<subseteq> \<lbrakk>\<lbrakk> \<Gamma>\<^sub>1 \<rbrakk>\<rbrakk>\<^sub>s\<^sub>y\<^sub>m\<^sub>r\<^sub>u\<^sub>n \<inter> \<lbrakk>\<lbrakk> \<Psi>\<^sub>1 \<nabla> n\<^sub>1 \<rbrakk>\<rbrakk>\<^sub>T\<^sub>E\<^sub>S\<^sub>L \<inter> \<lbrakk>\<lbrakk> \<Phi>\<^sub>1 \<nabla> Suc n\<^sub>1 \<rbrakk>\<rbrakk>\<^sub>T\<^sub>E\<^sub>S\<^sub>L"
+      using a1 a2 by auto
+    qed
   qed
+
+theorem reduction_refinement':
+  assumes "\<S>\<^sub>1 \<hookrightarrow> \<S>\<^sub>2"
+  shows "\<lbrakk> \<S>\<^sub>1 \<rbrakk>\<^sub>H\<^sub>e\<^sub>r\<^sub>o\<^sub>n \<supseteq> \<lbrakk> \<S>\<^sub>2 \<rbrakk>\<^sub>H\<^sub>e\<^sub>r\<^sub>o\<^sub>n"
+  by (metis reduction_refinement HeronConf_interpretation.elims assms)
+
+(* TODO: Need to show the same property for an arbitrary number of reduction steps*)
+(* Playing with [rel] type *)
+theorem reduction_refinement'':
+  assumes "(\<S>\<^sub>1, \<S>\<^sub>2) \<in> \<hookrightarrow>\<^sup>\<up>"
+  shows "\<lbrakk> \<S>\<^sub>1 \<rbrakk>\<^sub>H\<^sub>e\<^sub>r\<^sub>o\<^sub>n \<supseteq> \<lbrakk> \<S>\<^sub>2 \<rbrakk>\<^sub>H\<^sub>e\<^sub>r\<^sub>o\<^sub>n"
+  proof -
+    have "\<S>\<^sub>1 \<hookrightarrow> \<S>\<^sub>2" using assms by auto
+    then show ?thesis using reduction_refinement' by auto
+  qed
+
+theorem reduction_refinement_2:
+  assumes "(\<S>\<^sub>1, \<S>\<^sub>2) \<in> \<hookrightarrow>\<^sup>\<up> ^^ 2"
+  shows "\<lbrakk> \<S>\<^sub>1 \<rbrakk>\<^sub>H\<^sub>e\<^sub>r\<^sub>o\<^sub>n \<supseteq> \<lbrakk> \<S>\<^sub>2 \<rbrakk>\<^sub>H\<^sub>e\<^sub>r\<^sub>o\<^sub>n"
+  proof -
+    obtain \<S>' where "(\<S>\<^sub>1, \<S>') \<in> \<hookrightarrow>\<^sup>\<up> \<and> (\<S>', \<S>\<^sub>2) \<in> \<hookrightarrow>\<^sup>\<up>" sorry
+    have "\<S>\<^sub>1 \<hookrightarrow> \<S>\<^sub>2" using assms sorry
+    then show ?thesis using reduction_refinement' sorry
+  qed
+
+theorem reduction_refinement_general:
+  assumes "(\<S>\<^sub>1, \<S>\<^sub>2) \<in> (\<hookrightarrow>\<^sup>\<up> ^^ n)"
+  shows "\<lbrakk> \<S>\<^sub>1 \<rbrakk>\<^sub>H\<^sub>e\<^sub>r\<^sub>o\<^sub>n \<supseteq> \<lbrakk> \<S>\<^sub>2 \<rbrakk>\<^sub>H\<^sub>e\<^sub>r\<^sub>o\<^sub>n"
+  proof (induct n)
+    case 0
+    then have *: "(\<S>\<^sub>1, \<S>\<^sub>2) \<in> (\<hookrightarrow>\<^sup>\<up> ^^ 0) \<Longrightarrow> \<S>\<^sub>1 = \<S>\<^sub>2"
+      by auto
+    moreover have "\<S>\<^sub>1 = \<S>\<^sub>2" using *
+      sorry
+    ultimately show ?case by auto
+  next
+    case (Suc n)
+    then show ?case sorry
+  qed
+
+theorem
+  assumes "(\<S>\<^sub>1, \<S>\<^sub>2) \<in> \<hookrightarrow>\<^sup>\<up>\<^sup>*"
+  shows "\<lbrakk> \<S>\<^sub>1 \<rbrakk>\<^sub>H\<^sub>e\<^sub>r\<^sub>o\<^sub>n \<supseteq> \<lbrakk> \<S>\<^sub>2 \<rbrakk>\<^sub>H\<^sub>e\<^sub>r\<^sub>o\<^sub>n"
+  apply (insert assms)
+  proof -
+    have "\<S>\<^sub>1 = \<S>\<^sub>2 \<Longrightarrow> (\<S>\<^sub>1, \<S>\<^sub>2) \<in> \<hookrightarrow>\<^sup>\<up>\<^sup>* \<Longrightarrow> \<lbrakk> \<S>\<^sub>2 \<rbrakk>\<^sub>H\<^sub>e\<^sub>r\<^sub>o\<^sub>n \<subseteq> \<lbrakk> \<S>\<^sub>1 \<rbrakk>\<^sub>H\<^sub>e\<^sub>r\<^sub>o\<^sub>n "
+      by auto
+    moreover have "\<S>\<^sub>1 \<noteq> \<S>\<^sub>2 \<Longrightarrow> (\<S>\<^sub>1, \<S>\<^sub>2) \<in> \<hookrightarrow>\<^sup>\<up>\<^sup>* \<Longrightarrow> \<lbrakk> \<S>\<^sub>2 \<rbrakk>\<^sub>H\<^sub>e\<^sub>r\<^sub>o\<^sub>n \<subseteq> \<lbrakk> \<S>\<^sub>1 \<rbrakk>\<^sub>H\<^sub>e\<^sub>r\<^sub>o\<^sub>n"
+      (* apply (frule rtrancl_into_rtrancl) *)
+      proof -
+        have "undefined" sorry
+        show ?thesis sorry
+      qed
+    ultimately show ?thesis using assms by blast
+  qed
+
+(* To start solving specification [\<Psi>], we start at configuration [], 0 \<turnstile> \<Psi> \<triangleright> [] *)
+lemma solve_start:
+  shows "\<lbrakk>\<lbrakk> \<Psi> \<rbrakk>\<rbrakk>\<^sub>T\<^sub>E\<^sub>S\<^sub>L = \<lbrakk> [], 0 \<turnstile> \<Psi> \<triangleright> [] \<rbrakk>\<^sub>H\<^sub>e\<^sub>r\<^sub>o\<^sub>n"
+  proof -
+    have "\<lbrakk>\<lbrakk> \<Psi> \<rbrakk>\<rbrakk>\<^sub>T\<^sub>E\<^sub>S\<^sub>L = \<lbrakk>\<lbrakk> \<Psi> \<nabla> 0 \<rbrakk>\<rbrakk>\<^sub>T\<^sub>E\<^sub>S\<^sub>L"
+    by (simp add: TESL_interpretation_at_index_zero')
+    moreover have "\<lbrakk> [], 0 \<turnstile> \<Psi> \<triangleright> [] \<rbrakk>\<^sub>H\<^sub>e\<^sub>r\<^sub>o\<^sub>n = \<lbrakk>\<lbrakk> [] \<rbrakk>\<rbrakk>\<^sub>s\<^sub>y\<^sub>m\<^sub>r\<^sub>u\<^sub>n \<inter> \<lbrakk>\<lbrakk> \<Psi> \<nabla> 0 \<rbrakk>\<rbrakk>\<^sub>T\<^sub>E\<^sub>S\<^sub>L \<inter> \<lbrakk>\<lbrakk> [] \<nabla> Suc 0 \<rbrakk>\<rbrakk>\<^sub>T\<^sub>E\<^sub>S\<^sub>L"
+    by simp
+    ultimately show ?thesis by auto
+  qed
+
+(**) section \<open>Termination of instantataneous formulae elimination\<close> (**)
+(* Idea: A bounded monotonic sequence is convergent *)
+fun count_interpretation :: "TESL_formula \<Rightarrow> nat" ("\<lbrakk>\<lbrakk> _ \<rbrakk>\<rbrakk>\<^sub>c\<^sub>n\<^sub>t") where
+    "\<lbrakk>\<lbrakk> [] \<rbrakk>\<rbrakk>\<^sub>c\<^sub>n\<^sub>t = (0::nat)"
+  | "\<lbrakk>\<lbrakk> \<phi> # \<Phi> \<rbrakk>\<rbrakk>\<^sub>c\<^sub>n\<^sub>t = (case \<phi> of
+                        _ sporadic _ on _ \<Rightarrow> 1 + \<lbrakk>\<lbrakk> \<Phi> \<rbrakk>\<rbrakk>\<^sub>c\<^sub>n\<^sub>t
+                      | _                 \<Rightarrow> 2 + \<lbrakk>\<lbrakk> \<Phi> \<rbrakk>\<rbrakk>\<^sub>c\<^sub>n\<^sub>t)"
+lemma present_strictly_decreasing:
+  assumes "\<Gamma>\<^sub>1, n \<turnstile> \<Psi>\<^sub>1 \<triangleright> \<Phi>\<^sub>1  \<hookrightarrow>  \<Gamma>\<^sub>2, n \<turnstile> \<Psi>\<^sub>2 \<triangleright> \<Phi>\<^sub>2"
+  shows "\<lbrakk>\<lbrakk> \<Psi>\<^sub>1 \<rbrakk>\<rbrakk>\<^sub>c\<^sub>n\<^sub>t > \<lbrakk>\<lbrakk> \<Psi>\<^sub>2 \<rbrakk>\<rbrakk>\<^sub>c\<^sub>n\<^sub>t"
+  by (insert assms, erule operational_semantics_step.cases, auto)
 
 lemma run_index_progress:
   assumes "\<Gamma>\<^sub>1, n\<^sub>1 \<turnstile> \<Psi>\<^sub>1 \<triangleright> \<Phi>\<^sub>1  \<hookrightarrow>  \<Gamma>\<^sub>2, n\<^sub>2 \<turnstile> \<Psi>\<^sub>2 \<triangleright> \<Phi>\<^sub>2"
