Run.thy
@@ -34,8 +34,7 @@ lemma Abs_run_inverse_rewrite_unsafe:
 
 
 fun symbolic_run_interpretation_primitive :: "constr \<Rightarrow> run set" ("\<lbrakk> _ \<rbrakk>\<^sub>s\<^sub>y\<^sub>m\<^sub>r\<^sub>u\<^sub>n") where
-    "\<lbrakk> \<top>\<^sub>s\<^sub>y\<^sub>m\<^sub>r\<^sub>u\<^sub>n  \<rbrakk>\<^sub>s\<^sub>y\<^sub>m\<^sub>r\<^sub>u\<^sub>n  = { _. True }"
-  | "\<lbrakk> K \<Up> n  \<rbrakk>\<^sub>s\<^sub>y\<^sub>m\<^sub>r\<^sub>u\<^sub>n   = { \<rho>. hamlet ((Rep_run \<rho>) n K) = True }"
+    "\<lbrakk> K \<Up> n  \<rbrakk>\<^sub>s\<^sub>y\<^sub>m\<^sub>r\<^sub>u\<^sub>n   = { \<rho>. hamlet ((Rep_run \<rho>) n K) = True }"
   | "\<lbrakk> K \<not>\<Up> n \<rbrakk>\<^sub>s\<^sub>y\<^sub>m\<^sub>r\<^sub>u\<^sub>n   = { \<rho>. hamlet ((Rep_run \<rho>) n K) = False }"
   | "\<lbrakk> K \<Down> n @ \<lfloor> \<tau> \<rfloor> \<rbrakk>\<^sub>s\<^sub>y\<^sub>m\<^sub>r\<^sub>u\<^sub>n = { \<rho>. time ((Rep_run \<rho>) n K) = \<tau> }"
   | "\<lbrakk> K \<Down> n @ \<lfloor> \<tau>\<^sub>v\<^sub>a\<^sub>r(K', n') \<oplus> \<tau> \<rfloor> \<rbrakk>\<^sub>s\<^sub>y\<^sub>m\<^sub>r\<^sub>u\<^sub>n = { \<rho>. time ((Rep_run \<rho>) n K) = time ((Rep_run \<rho>) n' K') + \<tau> }"
@@ -65,8 +64,7 @@ fun time_update
 
 (* Update functionals *)
 fun run_update :: "run \<Rightarrow> constr \<Rightarrow> run" ("_ \<langle> _ \<rangle>") where
-    "\<rho> \<langle> \<top>\<^sub>s\<^sub>y\<^sub>m\<^sub>r\<^sub>u\<^sub>n \<rangle>  = \<rho>"
-  | "\<rho> \<langle> K \<Up> n \<rangle>  = Abs_run (\<lambda>n' K'. if K = K' \<and> n = n' then (True, time ((Rep_run \<rho>) n K)) else (Rep_run \<rho>) n' K')"
+    "\<rho> \<langle> K \<Up> n \<rangle>  = Abs_run (\<lambda>n' K'. if K = K' \<and> n = n' then (True, time ((Rep_run \<rho>) n K)) else (Rep_run \<rho>) n' K')"
   | "\<rho> \<langle> K \<not>\<Up> n \<rangle> = Abs_run (\<lambda>n' K'. if K = K' \<and> n = n' then (False, time ((Rep_run \<rho>) n K)) else (Rep_run \<rho>) n' K')"
   | "\<rho> \<langle> K \<Down> n @ \<lfloor> \<tau> \<rfloor> \<rangle> = Abs_run (time_update n K \<tau> (Rep_run \<rho>))"
   | "\<rho> \<langle> K \<Down> n @ \<lfloor> \<tau>\<^sub>v\<^sub>a\<^sub>r(K', n') \<oplus> \<tau> \<rfloor> \<rangle> =
@@ -271,9 +269,5 @@ lemma symrun_interp_absorb2:
   assumes incl: "set \<Gamma>\<^sub>2 \<subseteq> set \<Gamma>\<^sub>1"
   shows "\<lbrakk>\<lbrakk> \<Gamma>\<^sub>1 @ \<Gamma>\<^sub>2 \<rbrakk>\<rbrakk>\<^sub>s\<^sub>y\<^sub>m\<^sub>r\<^sub>u\<^sub>n = \<lbrakk>\<lbrakk> \<Gamma>\<^sub>1 \<rbrakk>\<rbrakk>\<^sub>s\<^sub>y\<^sub>m\<^sub>r\<^sub>u\<^sub>n"
   using symrun_interp_absorb1 symrun_interp_commute incl by blast
-
-lemma TrueSymrun_idem:
-  "\<lbrakk>\<lbrakk> \<top>\<^sub>s\<^sub>y\<^sub>m\<^sub>r\<^sub>u\<^sub>n # \<Gamma> \<rbrakk>\<rbrakk>\<^sub>s\<^sub>y\<^sub>m\<^sub>r\<^sub>u\<^sub>n = \<lbrakk>\<lbrakk> \<Gamma> \<rbrakk>\<rbrakk>\<^sub>s\<^sub>y\<^sub>m\<^sub>r\<^sub>u\<^sub>n"
-  by auto
 
 end
